Prove first chunk of inference soundness

typing/pure_inferenceProofScript.sml
@@ -875,6 +875,1426 @@ QED
 
 (******************** Main results ********************)
 
+Definition ctxt_rel_def:
+  ctxt_rel tdefs sub as ctxt ⇔
+    ∀k v. FLOOKUP as k = SOME v ⇒
+      ∃vars scheme.
+        ALOOKUP ctxt k = SOME (vars,scheme) ∧
+        ∀n. n ∈ v ⇒
+          ∃inst. LENGTH inst = vars ∧
+            EVERY (λit. itype_ok tdefs 0 it ∧
+                        pure_vars it ⊆ pure_vars (pure_walkstar sub (CVar n))) inst ∧
+            isubst inst (pure_walkstar sub scheme) = pure_walkstar sub (CVar n)
+End
+
+Theorem ctxt_rel_mInstantiate:
+  pure_wfs sub ∧
+  ctxt_rel tdefs sub as ctxt ⇒
+    ∀k v. FLOOKUP as k = SOME v ⇒
+      ∃vars scheme. ALOOKUP ctxt k = SOME (vars,scheme) ∧
+        ∀n. n ∈ v ⇒
+          satisfies tdefs sub $ mInstantiate (CVar n) (vars, scheme)
+Proof
+  rw[ctxt_rel_def] >> first_x_assum drule >> rw[] >> simp[] >>
+  rw[] >> first_x_assum drule >> rw[satisfies_def] >>
+  irule_at Any EQ_REFL >> simp[] >> gvs[EVERY_MEM]
+QED
+
+Theorem ctxt_rel_sub:
+  ∀tdefs sub as ctxt as'.
+    ctxt_rel tdefs sub as ctxt ∧
+    (∀k v. FLOOKUP as' k = SOME v ⇒ ∃v'. FLOOKUP as k = SOME v' ∧ v ⊆ v')
+  ⇒ ctxt_rel tdefs sub as' ctxt
+Proof
+  rw[ctxt_rel_def] >> first_x_assum drule >> rw[] >>
+  first_x_assum drule >> rw[] >> simp[] >> rw[] >> gvs[SUBSET_DEF]
+QED
+
+Theorem inference_constraints_sound:
+  ∀ns sub.
+    namespace_ok ns ∧
+    pure_wfs sub ∧
+    (∀it. it ∈ FRANGE sub ⇒ itype_ok (SND ns) 0 it) ⇒
+  ∀mset cexp as cs it ictxt ctxt db closing t.
+    minfer ns mset cexp as cs it ∧
+    FINITE mset ∧
+    (∀c. c ∈ cs ⇒ satisfies (SND ns) sub c) ∧
+    ctxt_rel (SND ns) sub as ictxt ∧
+    EVERY (λ(x,vs,it). freedbvars it ⊆ count vs) ictxt ∧
+    msubst_vars sub (ctxt_vars ictxt) = msubst_vars sub mset ∧
+    (∀n. n ∈ new_vars as cs it ⇒
+      pure_vars (pure_walkstar sub (CVar n)) ⊆ FDOM closing) ∧
+    (∀it. it ∈ FRANGE closing ⇒ pure_vars it = {} ∧ itype_ok (SND ns) db it) ∧
+    LIST_REL (λ(xs,vs,t) (ixs,ivs,it). xs = ixs ∧ vs = ivs ∧
+      type_of $ csubst (ishift vs o_f closing) (pure_walkstar sub it) = SOME t)
+      ctxt ictxt ∧
+    type_of $ csubst closing (pure_walkstar sub it) = SOME t
+    ⇒ type_tcexp ns db [] ctxt (tcexp_of cexp) t
+Proof
+  rpt gen_tac >> strip_tac >>
+  ntac 5 gen_tac >> Induct_on `minfer` >> rw[tcexp_of_def] >> gvs[]
+  >- ( (* Var *)
+    simp[Once type_tcexp_cases] >> gvs[ctxt_rel_def, FLOOKUP_UPDATE] >>
+    qspecl_then [`ictxt`,`ctxt`] mp_tac ALOOKUP_SOME_EL_2 >>
+    disch_then drule >> gvs[LIST_REL_EL_EQN] >> impl_tac
+    >- (
+      rw[Once LIST_EQ_REWRITE, EL_MAP] >>
+      first_x_assum drule >> rpt (pairarg_tac >> simp[])
+      ) >>
+    strip_tac >> gvs[] >> rename1 `_ = (v,s)` >> PairCases_on `s` >>
+    first_x_assum drule >> rw[specialises_def] >>
+    `EVERY (λit. pure_vars it = {}) (MAP (csubst closing) inst)` by (
+      gvs[EVERY_MAP, EVERY_MEM] >> rw[] >>
+      first_x_assum drule >> rw[] >>
+      simp[pure_vars_pure_apply_subst] >> rw[IMAGE_EQ_SING, DISJ_EQ_IMP] >>
+      simp[pure_apply_subst] >> reverse CASE_TAC >> gvs[pure_vars]
+      >- (gvs[IN_FRANGE_FLOOKUP, PULL_EXISTS] >> first_x_assum drule >> simp[]) >>
+      gvs[new_vars_def, pure_vars] >> gvs[FLOOKUP_DEF, SUBSET_DEF]) >>
+    gvs[pure_vars_empty_eq_type_of_MAP] >>
+    qexists_tac `ts` >> rw[] >> gvs[]
+    >- (
+      gvs[MAP_EQ_EVERY2, EVERY_EL, LIST_REL_EL_EQN] >> rw[] >>
+      simp[GSYM itype_ok_type_ok] >> first_x_assum drule >> rw[EL_MAP] >>
+      drule type_of_SOME >> rw[] >>
+      irule itype_ok_pure_apply_subst >> simp[] >>
+      last_x_assum drule >> rw[] >> gvs[itype_ok_def]
+      )
+    >- gvs[MAP_EQ_EVERY2] >>
+    simp[GSYM itype_of_11, GSYM isubst_itype_of] >>
+    drule type_of_SOME_MAP >> rw[] >>
+    imp_res_tac type_of_SOME >> rw[] >>
+    simp[GSYM pure_apply_subst_isubst_strong]
+    )
+  >- ( (* Tuple *)
+    simp[Once type_tcexp_cases] >> disj1_tac >>
+    gvs[pure_walkstar_alt, pure_apply_subst] >>
+    imp_res_tac $ cj 1 type_of_SOME_lemma >> gvs[] >>
+    gvs[LIST_REL_EL_EQN, EL_ZIP, EL_MAP, MAP_EQ_EVERY2] >> rw[] >>
+    last_x_assum drule >> strip_tac >> pop_assum irule >> conj_tac
+    >- (rw[] >> first_x_assum irule >> goal_assum drule >> simp[EL_MEM]) >>
+    rpt $ goal_assum $ drule_at Any >> simp[] >> rw[]
+    >- (
+      gvs[GSYM pure_walkstar_alt] >> first_x_assum irule >>
+      irule new_vars_SUBSET >> goal_assum drule >>
+      irule_at Any BIGUNION_FRANGE_FOLDR_maunion >> simp[EL_MEM] >>
+      simp[pure_vars, SUBSET_DEF, MEM_MAP, MEM_EL, PULL_EXISTS, SF SFY_ss]
+      )
+    >- (
+      irule ctxt_rel_sub >> goal_assum $ drule_at Any >> rw[] >>
+      simp[FLOOKUP_FOLDR_maunion, MEM_EL, PULL_EXISTS, GSYM CONJ_ASSOC] >>
+      goal_assum drule >> gvs[FLOOKUP_DEF] >>
+      simp[SUBSET_DEF, PULL_EXISTS, SF SFY_ss]
+      )
+    )
+  >- ( (* Ret *)
+    simp[Once type_tcexp_cases] >> disj1_tac >>
+    gvs[pure_walkstar_alt, pure_apply_subst, type_of_def] >>
+    last_x_assum irule >> rpt $ goal_assum $ drule_at Any >>
+    gvs[GSYM pure_walkstar_alt] >> rw[] >>
+    first_x_assum irule >> irule new_vars_SUBSET >>
+    goal_assum drule >> simp[pure_vars]
+    )
+  >- ( (* Bind *)
+    simp[Once type_tcexp_cases] >> disj1_tac >>
+    gvs[DISJ_IMP_THM, FORALL_AND_THM, satisfies_def] >>
+    gvs[pure_walkstar_alt, pure_apply_subst, type_of_def] >>
+    ntac 2 $ last_x_assum $ irule_at Any >> rpt $ goal_assum $ drule_at Any >>
+    gvs[GSYM pure_walkstar_alt] >>
+    `pure_vars (csubst closing (pure_walkstar sub (CVar f1))) = {}` by (
+      irule pure_vars_csubst_EMPTY_suff >> simp[] >>
+      first_x_assum irule >> simp[new_vars_def, pure_vars]) >>
+    gvs[pure_vars_empty_eq_type_of] >> rw[]
+    >- (
+      irule ctxt_rel_sub >> goal_assum $ drule_at Any >>
+      rw[FLOOKUP_maunion] >> CASE_TAC >> simp[]
+      )
+    >- (
+      first_x_assum irule >> irule new_vars_SUBSET_minfer >> goal_assum drule >>
+      simp[BIGUNION_FRANGE_maunion] >> imp_res_tac minfer_pure_vars
+      )
+    >- (
+      irule ctxt_rel_sub >> goal_assum $ drule_at Any >>
+      rw[FLOOKUP_maunion] >> CASE_TAC >> simp[]
+      )
+    >- (
+      first_x_assum irule >> irule new_vars_SUBSET_minfer >> goal_assum drule >>
+      simp[BIGUNION_FRANGE_maunion] >> imp_res_tac minfer_pure_vars >> simp[SUBSET_DEF]
+      )
+    )
+  >- ( (* Raise *)
+    simp[Once type_tcexp_cases] >> disj1_tac >>
+    gvs[DISJ_IMP_THM, FORALL_AND_THM, satisfies_def] >>
+    gvs[pure_walkstar_alt, pure_apply_subst, type_of_def] >>
+    gvs[GSYM pure_walkstar_alt] >>
+    last_x_assum $ irule_at Any >> rpt $ goal_assum $ drule_at Any >> rw[]
+    >- (
+      first_x_assum irule >> irule new_vars_SUBSET_minfer >> goal_assum drule >>
+      simp[] >> imp_res_tac minfer_pure_vars >> simp[SUBSET_DEF]
+      )
+    >- (
+      imp_res_tac type_of_SOME >> simp[GSYM itype_ok_type_ok] >>
+      irule itype_ok_pure_apply_subst >> simp[] >>
+      irule itype_ok_pure_walkstar >> rw[itype_ok] >> gvs[itype_ok_def]
+      )
+    )
+  >- ( (* Handle *)
+    simp[Once type_tcexp_cases] >> disj1_tac >>
+    gvs[DISJ_IMP_THM, FORALL_AND_THM, satisfies_def] >>
+    gvs[pure_walkstar_alt, pure_apply_subst, type_of_def] >>
+    ntac 2 $ last_x_assum $ irule_at Any >> rpt $ goal_assum $ drule_at Any >>
+    gvs[GSYM pure_walkstar_alt] >> rw[]
+    >- (
+      irule ctxt_rel_sub >> goal_assum $ drule_at Any >>
+      rw[FLOOKUP_maunion] >> CASE_TAC >> simp[]
+      )
+    >- (
+      first_x_assum irule >> irule new_vars_SUBSET_minfer >> goal_assum drule >>
+      simp[BIGUNION_FRANGE_maunion] >> imp_res_tac minfer_pure_vars
+      )
+    >- (
+      irule ctxt_rel_sub >> goal_assum $ drule_at Any >>
+      rw[FLOOKUP_maunion] >> CASE_TAC >> simp[]
+      )
+    >- (
+      first_x_assum irule >> irule new_vars_SUBSET_minfer >> goal_assum drule >>
+      simp[BIGUNION_FRANGE_maunion] >> imp_res_tac minfer_pure_vars >> simp[SUBSET_DEF]
+      )
+    )
+  >- ( (* Act *)
+    simp[Once type_tcexp_cases] >> disj1_tac >>
+    gvs[DISJ_IMP_THM, FORALL_AND_THM, satisfies_def] >>
+    gvs[pure_walkstar_alt, pure_apply_subst, type_of_def] >>
+    last_x_assum irule >> rpt $ goal_assum $ drule_at Any >> rw[] >>
+    gvs[GSYM pure_walkstar_alt] >>
+    first_x_assum irule >> irule new_vars_SUBSET_minfer >> goal_assum drule >>
+    imp_res_tac minfer_pure_vars >> simp[SUBSET_DEF]
+    )
+  >- ( (* Alloc *)
+    simp[Once type_tcexp_cases] >> disj1_tac >>
+    gvs[DISJ_IMP_THM, FORALL_AND_THM, satisfies_def] >>
+    gvs[pure_walkstar_alt, pure_apply_subst, type_of_def] >>
+    ntac 2 $ last_x_assum $ irule_at Any >> rpt $ goal_assum $ drule_at Any >>
+    gvs[GSYM pure_walkstar_alt] >> rw[]
+    >- (
+      irule ctxt_rel_sub >> goal_assum $ drule_at Any >>
+      rw[FLOOKUP_maunion] >> CASE_TAC >> simp[]
+      )
+    >- (
+      first_x_assum irule >> irule new_vars_SUBSET_minfer >> goal_assum drule >>
+      simp[BIGUNION_FRANGE_maunion] >> imp_res_tac minfer_pure_vars >> simp[SUBSET_DEF]
+      )
+    >- (
+      irule ctxt_rel_sub >> goal_assum $ drule_at Any >>
+      rw[FLOOKUP_maunion] >> CASE_TAC >> simp[]
+      )
+    >- (
+      first_x_assum irule >> irule new_vars_SUBSET_minfer >> goal_assum drule >>
+      simp[BIGUNION_FRANGE_maunion] >> imp_res_tac minfer_pure_vars >> simp[SUBSET_DEF]
+      )
+    )
+  >- ( (* Length *)
+    simp[Once type_tcexp_cases] >> disj1_tac >>
+    gvs[DISJ_IMP_THM, FORALL_AND_THM, satisfies_def] >>
+    gvs[pure_walkstar_alt, pure_apply_subst, type_of_def] >>
+    last_x_assum $ irule_at Any >> rpt $ goal_assum $ drule_at Any >>
+    gvs[GSYM pure_walkstar_alt] >>
+    `pure_vars (csubst closing (pure_walkstar sub (CVar fresh))) = {}` by (
+      irule pure_vars_csubst_EMPTY_suff >> simp[] >>
+      first_x_assum irule >> simp[new_vars_def, pure_vars]) >>
+    gvs[pure_vars_empty_eq_type_of] >> rw[] >>
+    first_x_assum irule >> irule new_vars_SUBSET_minfer >> goal_assum drule >>
+    imp_res_tac minfer_pure_vars >> simp[SUBSET_DEF]
+    )
+  >- ( (* Deref *)
+    simp[Once type_tcexp_cases] >> disj1_tac >>
+    gvs[DISJ_IMP_THM, FORALL_AND_THM, satisfies_def] >>
+    gvs[pure_walkstar_alt, pure_apply_subst, type_of_def] >>
+    ntac 2 $ last_x_assum $ irule_at Any >> rpt $ goal_assum $ drule_at Any >>
+    gvs[GSYM pure_walkstar_alt] >> rw[]
+    >- (
+      irule ctxt_rel_sub >> goal_assum $ drule_at Any >>
+      rw[FLOOKUP_maunion] >> CASE_TAC >> simp[]
+      )
+    >- (
+      first_x_assum irule >> irule new_vars_SUBSET_minfer >> goal_assum drule >>
+      simp[BIGUNION_FRANGE_maunion] >> imp_res_tac minfer_pure_vars >> simp[SUBSET_DEF]
+      )
+    >- (
+      irule ctxt_rel_sub >> goal_assum $ drule_at Any >>
+      rw[FLOOKUP_maunion] >> CASE_TAC >> simp[]
+      )
+    >- (
+      first_x_assum irule >> irule new_vars_SUBSET_minfer >> goal_assum drule >>
+      simp[BIGUNION_FRANGE_maunion] >> imp_res_tac minfer_pure_vars >> simp[SUBSET_DEF]
+      )
+    )
+  >- ( (* Update *)
+    simp[Once type_tcexp_cases] >> disj1_tac >>
+    gvs[DISJ_IMP_THM, FORALL_AND_THM, satisfies_def] >>
+    gvs[pure_walkstar_alt, pure_apply_subst, type_of_def] >>
+    ntac 3 $ last_x_assum $ irule_at Any >> rpt $ goal_assum $ drule_at Any >>
+    gvs[GSYM pure_walkstar_alt] >>
+    `pure_vars (csubst closing (pure_walkstar sub (CVar f))) = {}` by (
+      irule pure_vars_csubst_EMPTY_suff >> simp[] >>
+      first_x_assum irule >> simp[new_vars_def, pure_vars]) >>
+    gvs[pure_vars_empty_eq_type_of] >> rw[]
+    >- (
+      irule ctxt_rel_sub >> goal_assum $ drule_at Any >>
+      rw[FLOOKUP_maunion] >> rpt CASE_TAC >> simp[SUBSET_DEF]
+      )
+    >- (
+      first_x_assum irule >> irule new_vars_SUBSET_minfer >> goal_assum drule >>
+      simp[BIGUNION_FRANGE_maunion] >> imp_res_tac minfer_pure_vars >> simp[SUBSET_DEF]
+      )
+    >- (
+      irule ctxt_rel_sub >> goal_assum $ drule_at Any >>
+      rw[FLOOKUP_maunion] >> rpt CASE_TAC >> simp[SUBSET_DEF]
+      )
+    >- (
+      first_x_assum irule >> irule new_vars_SUBSET_minfer >> goal_assum drule >>
+      simp[BIGUNION_FRANGE_maunion] >> imp_res_tac minfer_pure_vars >> simp[SUBSET_DEF]
+      )
+    >- (
+      irule ctxt_rel_sub >> goal_assum $ drule_at Any >>
+      rw[FLOOKUP_maunion] >> rpt CASE_TAC >> simp[SUBSET_DEF]
+      )
+    >- (
+      first_x_assum irule >> irule new_vars_SUBSET_minfer >> goal_assum drule >>
+      simp[BIGUNION_FRANGE_maunion] >> imp_res_tac minfer_pure_vars >> simp[SUBSET_DEF]
+      )
+    )
+  >- ( (* True *)
+    simp[Once type_tcexp_cases] >>
+    gvs[pure_walkstar_alt, pure_apply_subst, type_of_def]
+    )
+  >- ( (* False *)
+    simp[Once type_tcexp_cases] >>
+    gvs[pure_walkstar_alt, pure_apply_subst, type_of_def]
+    )
+  >- ( (* Subscript *)
+    simp[Once type_tcexp_cases] >>
+    gvs[pure_walkstar_alt, pure_apply_subst, type_of_def]
+    )
+  >- ( (* Exception *)
+    simp[Once type_tcexp_cases] >>
+    gvs[DISJ_IMP_THM, FORALL_AND_THM, satisfies_def] >>
+    gvs[pure_walkstar_alt, pure_apply_subst, type_of_def] >>
+    `s ≠ "Subscript"` by gvs[pure_configTheory.reserved_cns_def] >> simp[] >>
+    PairCases_on `ns` >> gvs[] >> simp[type_exception_def] >>
+    gvs[LIST_REL_EL_EQN, EL_ZIP, EL_MAP] >> rw[] >>
+    last_x_assum drule >> strip_tac >> pop_assum irule >> conj_tac
+    >- gvs[MEM_EL, PULL_EXISTS, SF SFY_ss] >>
+    rpt $ goal_assum $ drule_at Any >> gvs[] >>
+    gvs[MAP2_MAP, MEM_MAP, MEM_ZIP, PULL_EXISTS, satisfies_def, type_of_itype_of] >>
+    gvs[GSYM pure_walkstar_alt] >> rw[]
+    >- (
+      first_x_assum irule >> irule new_vars_SUBSET_minfer >> goal_assum drule >>
+      irule_at Any BIGUNION_FRANGE_FOLDR_maunion >> simp[EL_MEM] >>
+      imp_res_tac minfer_pure_vars >> simp[SUBSET_DEF, MEM_EL, SF SFY_ss, PULL_EXISTS]
+      )
+    >- (
+      irule ctxt_rel_sub >> goal_assum $ drule_at Any >> rw[] >>
+      simp[FLOOKUP_FOLDR_maunion, MEM_EL, PULL_EXISTS] >>
+      goal_assum drule >> gvs[FLOOKUP_DEF, SUBSET_DEF, PULL_EXISTS, SF SFY_ss]
+      )
+    )
+  >- ( (* Cons *)
+    simp[Once type_tcexp_cases] >>
+    gvs[DISJ_IMP_THM, FORALL_AND_THM, satisfies_def] >>
+    gvs[pure_walkstar_alt, pure_apply_subst] >>
+    drule $ cj 2 type_of_SOME_lemma >> rw[] >>
+    PairCases_on `ns` >> gvs[] >> simp[type_cons_def, PULL_EXISTS, oEL_THM] >>
+    gvs[LIST_REL_EL_EQN, MAP_EQ_EVERY2, EL_ZIP, EL_MAP] >> reverse $ rw[]
+    >- (
+      gvs[EVERY_EL] >> rw[] >> first_x_assum drule >> strip_tac >>
+      imp_res_tac type_of_SOME >> simp[GSYM itype_ok_type_ok] >>
+      irule itype_ok_pure_apply_subst >> simp[] >>
+      irule itype_ok_pure_walkstar >> simp[itype_ok] >> gvs[itype_ok_def]
+      ) >>
+    last_x_assum drule >> strip_tac >> pop_assum irule >> conj_tac
+    >- gvs[MEM_EL, PULL_EXISTS, SF SFY_ss] >>
+    rpt $ goal_assum $ drule_at Any >> gvs[GSYM pure_walkstar_alt] >> rw[]
+    >- (
+      first_x_assum irule >> irule new_vars_SUBSET_minfer >> goal_assum drule >>
+      irule_at Any BIGUNION_FRANGE_FOLDR_maunion >> simp[EL_MEM] >>
+      imp_res_tac minfer_pure_vars >> simp[SUBSET_DEF, MEM_EL, SF SFY_ss, PULL_EXISTS]
+      )
+    >- (
+      gvs[MAP2_MAP, MEM_MAP, MEM_ZIP, PULL_EXISTS, satisfies_def] >>
+      DEP_REWRITE_TAC[pure_walkstar_isubst] >> conj_tac >- gvs[itype_ok_def] >>
+      simp[pure_walkstar_itype_of, pure_apply_subst_isubst_itype_of] >>
+      drule $ cj 2 type_of_SOME_lemma >> rw[] >>
+      imp_res_tac type_of_SOME_MAP >> pop_assum $ assume_tac o GSYM >>
+      simp[isubst_itype_of, type_of_itype_of]
+      )
+    >- (
+      irule ctxt_rel_sub >> goal_assum $ drule_at Any >> rw[] >>
+      simp[FLOOKUP_FOLDR_maunion, MEM_EL, PULL_EXISTS] >>
+      goal_assum drule >> gvs[FLOOKUP_DEF, SUBSET_DEF, PULL_EXISTS, SF SFY_ss]
+      )
+    )
+  >- ( (* AtomOp *)
+    simp[Once type_tcexp_cases] >> disj2_tac >>
+    gvs[DISJ_IMP_THM, FORALL_AND_THM] >>
+    gvs[pure_walkstar_alt, pure_apply_subst, type_of_def] >>
+    gvs[GSYM pure_walkstar_alt] >>
+    imp_res_tac infer_atom_op_LENGTH >> pop_assum $ assume_tac o GSYM >> gvs[] >>
+    simp[GSYM infer_atom_op] >> goal_assum $ drule_at Any >> simp[get_PrimTys_SOME] >>
+    gvs[LIST_REL_EL_EQN, EL_ZIP, EL_MAP, MAP2_MAP, MEM_MAP, MEM_ZIP, PULL_EXISTS] >>
+    rw[] >> last_x_assum drule >> strip_tac >> pop_assum irule >> conj_tac
+    >- gvs[MEM_EL, PULL_EXISTS, SF SFY_ss] >>
+    rpt $ goal_assum $ drule_at Any >> gvs[satisfies_def] >>
+    simp[pure_walkstar_alt, pure_apply_subst, type_of_def] >> rw[GSYM pure_walkstar_alt]
+    >- (
+      first_x_assum irule >> irule new_vars_SUBSET_minfer >> goal_assum drule >>
+      irule_at Any BIGUNION_FRANGE_FOLDR_maunion >> simp[EL_MEM] >>
+      imp_res_tac minfer_pure_vars >> simp[SUBSET_DEF, MEM_EL, SF SFY_ss, PULL_EXISTS]
+      )
+    >- (
+      irule ctxt_rel_sub >> goal_assum $ drule_at Any >> rw[] >>
+      simp[FLOOKUP_FOLDR_maunion, MEM_EL, PULL_EXISTS] >>
+      goal_assum drule >> gvs[FLOOKUP_DEF, SUBSET_DEF, PULL_EXISTS, SF SFY_ss]
+      )
+    )
+  >- ( (* Seq *)
+    simp[Once type_tcexp_cases] >>
+    ntac 2 $ last_x_assum $ irule_at Any >> rpt $ goal_assum $ drule_at Any >>
+    `pure_vars (csubst closing (pure_walkstar sub it)) = {}` by (
+      irule pure_vars_csubst_EMPTY_suff >> simp[] >>
+      simp[pure_vars_pure_walkstar_alt] >> rw[BIGUNION_SUBSET, PULL_EXISTS] >>
+      first_x_assum irule >> imp_res_tac minfer_pure_vars >>
+      gvs[SUBSET_DEF, BIGUNION_FRANGE_maunion, new_vars_def, pure_vars] >>
+      metis_tac[]) >>
+    gvs[pure_vars_empty_eq_type_of] >> rw[]
+    >- (
+      irule ctxt_rel_sub >> goal_assum $ drule_at Any >>
+      rw[FLOOKUP_maunion] >> CASE_TAC >> simp[]
+      )
+    >- (
+      first_x_assum irule >> irule new_vars_SUBSET_minfer >> goal_assum drule >>
+      simp[BIGUNION_FRANGE_maunion] >> imp_res_tac minfer_pure_vars >> simp[SUBSET_DEF]
+      )
+    >- (
+      irule ctxt_rel_sub >> goal_assum $ drule_at Any >>
+      rw[FLOOKUP_maunion] >> CASE_TAC >> simp[]
+      )
+    >- (
+      first_x_assum irule >> irule new_vars_SUBSET_minfer >> goal_assum drule >>
+      simp[BIGUNION_FRANGE_maunion] >> imp_res_tac minfer_pure_vars >> simp[SUBSET_DEF]
+      )
+    )
+  >- ( (* App *)
+    simp[Once type_tcexp_cases] >>
+    gvs[DISJ_IMP_THM, FORALL_AND_THM, satisfies_def] >>
+    gvs[pure_walkstar_iFunctions, pure_apply_subst_iFunctions] >>
+    last_x_assum $ irule_at Any >> rpt $ goal_assum $ drule_at Any >>
+    irule_at Any $ cj 3 type_of_lemma >> simp[] >>
+    `EVERY (λit. pure_vars it = {})
+      (MAP (csubst closing) (MAP (pure_walkstar sub) tys))` by (
+      rw[EVERY_MAP, EVERY_MEM] >> irule pure_vars_csubst_EMPTY_suff >> simp[] >>
+      simp[pure_vars_pure_walkstar_alt] >> rw[BIGUNION_SUBSET, PULL_EXISTS] >>
+      rw[] >> first_x_assum irule >> simp[new_vars_def, pure_vars_iFunctions] >>
+      simp[MEM_MAP, PULL_EXISTS, SF SFY_ss]) >>
+    gvs[pure_vars_empty_eq_type_of_MAP] >> irule_at Any EQ_REFL >>
+    `ts ≠ []` by (CCONTR_TAC >> gvs[]) >> rw[]
+    >- (
+      irule ctxt_rel_sub >> goal_assum $ drule_at Any >>
+      rw[FLOOKUP_maunion] >> CASE_TAC >> simp[]
+      )
+    >- (
+      first_x_assum irule >> irule new_vars_SUBSET_minfer >>
+      goal_assum drule >> simp[BIGUNION_FRANGE_maunion] >>
+      imp_res_tac minfer_pure_vars >> simp[SUBSET_DEF]
+      ) >>
+    gvs[LIST_REL_EL_EQN, EL_ZIP, EL_MAP, MAP_EQ_EVERY2] >> rw[] >>
+    last_x_assum drule >> strip_tac >> pop_assum irule >> conj_tac
+    >- gvs[MEM_EL, PULL_EXISTS, SF SFY_ss] >>
+    rpt $ goal_assum $ drule_at Any >> rw[]
+    >- (
+      first_x_assum irule >> irule new_vars_SUBSET >>
+      qexistsl_tac [`FOLDR maunion FEMPTY ass`,`BIGUNION (set css)`,`CVar f`] >>
+      reverse $ conj_tac >- (simp[BIGUNION_FRANGE_maunion] >> simp[SUBSET_DEF]) >>
+      irule new_vars_SUBSET_minfer >> goal_assum drule >>
+      irule_at Any BIGUNION_FRANGE_FOLDR_maunion >> simp[EL_MEM] >>
+      imp_res_tac minfer_pure_vars >>
+      simp[SUBSET_DEF, MEM_EL, PULL_EXISTS, SF SFY_ss]
+      )
+    >- (
+      irule ctxt_rel_sub >> goal_assum $ drule_at Any >> rw[] >>
+      simp[FLOOKUP_maunion, FLOOKUP_FOLDR_maunion, MEM_EL, PULL_EXISTS] >>
+      rpt CASE_TAC >> gvs[FLOOKUP_DEF, SUBSET_DEF, PULL_EXISTS, SF SFY_ss]
+      )
+    )
+  >- ( (* Lam *)
+    simp[Once type_tcexp_cases] >>
+    gvs[pure_walkstar_iFunctions, pure_apply_subst_iFunctions] >>
+    drule $ cj 3 type_of_SOME_lemma >> rw[] >>
+    irule_at Any EQ_REFL >> simp[] >> rw[] >>
+    imp_res_tac $ cj 1 $ iffLR MAP_EQ_EVERY2 >> gvs[] >>
+    `ts ≠ []` by (CCONTR_TAC >> gvs[]) >> rw[]
+    >- (
+      gvs[EVERY_EL, MAP_EQ_EVERY2, LIST_REL_EL_EQN, EL_MAP] >> rw[] >>
+      first_x_assum drule >> strip_tac >>
+      imp_res_tac type_of_SOME >> simp[GSYM itype_ok_type_ok] >>
+      irule itype_ok_pure_apply_subst >> simp[] >>
+      irule itype_ok_pure_walkstar >> simp[itype_ok] >> gvs[itype_ok_def]
+      ) >>
+    last_x_assum irule >> goal_assum $ drule_at Any >> simp[] >>
+    qexists_tac `REVERSE (ZIP (xs, MAP ($, 0) (MAP CVar freshes))) ++ ictxt` >> rw[]
+    >- (
+      first_x_assum irule >> pop_assum mp_tac >>
+      simp[new_vars_def, PULL_EXISTS, pure_vars, IN_FRANGE_FLOOKUP,
+           FLOOKUP_FDIFF, MEM_MAP, GSYM DISJ_ASSOC, get_massumptions_def,
+           MAP2_MAP, MEM_ZIP, pure_vars_iFunctions] >>
+      reverse $ rw[] >> simp[SF SFY_ss] >>
+      reverse $ Cases_on `MEM k xs` >> gvs[] >> simp[SF SFY_ss] >>
+      pop_assum mp_tac >> simp[Once MEM_EL] >> strip_tac >> gvs[] >>
+      ntac 3 disj2_tac >> disj1_tac >>
+      rpt (goal_assum $ drule_at Any >> simp[])
+      )
+    >- (
+      simp[ctxt_vars, msubst_vars_UNION] >>
+      AP_THM_TAC >> AP_TERM_TAC >> simp[GSYM ctxt_vars_subst_ctxt] >>
+      simp[subst_ctxt_def, ctxt_vars_def, msubst_vars_def] >>
+      simp[MAP_REVERSE, ZIP_MAP] >>
+      simp[MAP_MAP_o, combinTheory.o_DEF, LAMBDA_PROD, MAP_ZIP_ALT] >>
+      AP_TERM_TAC >> rw[Once EXTENSION] >>
+      simp[MEM_MAP, MEM_ZIP, PULL_EXISTS, MEM_EL]
+      )
+    >- gvs[ZIP_MAP, EVERY_MAP, freedbvars_def]
+    >- (
+      gvs[MAP_EQ_EVERY2, LIST_REL_EL_EQN, EL_APPEND_EQN] >> rw[] >>
+      simp[ZIP_MAP, GSYM MAP_REVERSE, EL_MAP, EL_REVERSE, EL_ZIP] >> gvs[EL_MAP]
+      )
+    >- (
+      gvs[ctxt_rel_def] >> rw[] >> simp[ALOOKUP_APPEND] >> CASE_TAC
+      >- (
+        first_x_assum $ qspec_then `k` mp_tac >> simp[FLOOKUP_FDIFF] >>
+        impl_tac >> rw[] >> gvs[ALOOKUP_NONE, MAP_REVERSE, MAP_ZIP]
+        ) >>
+      PairCases_on `x` >> simp[] >> rw[] >>
+      imp_res_tac ALOOKUP_MEM >> gvs[MEM_ZIP, MEM_MAP, EL_MAP] >>
+      gvs[DISJ_IMP_THM, FORALL_AND_THM, PULL_EXISTS, MAP2_MAP, MEM_MAP, MEM_ZIP] >>
+      first_x_assum $ drule_at Any >> simp[get_massumptions_def] >>
+      disch_then drule >> simp[satisfies_def]
+      )
+    )
+  >- ( (* Let *)
+    rename [`Let _ (_ e1) (_ e2)`,
+            `minfer _ _ e2 as2 cs2 it2`,`minfer _ _ e1 as1 cs1 it1`] >>
+    simp[Once type_tcexp_cases] >>
+    last_x_assum $ irule_at Any >> goal_assum $ drule_at Any >>
+    `∃smonos : num_set. domain smonos = msubst_vars sub mset ∧ wf smonos` by (
+      qexists_tac `list_to_num_set (SET_TO_LIST (msubst_vars sub mset))` >>
+      simp[EXTENSION, domain_list_to_num_set, wf_list_to_num_set] >>
+      DEP_REWRITE_TAC[MEM_SET_TO_LIST] >> simp[msubst_vars_def, PULL_EXISTS]) >>
+    qabbrev_tac `gen = generalise 0 smonos FEMPTY (pure_walkstar sub it1)` >>
+    PairCases_on `gen` >> gvs[] >> rename1 `(new_dbvars,gen_sub,let_ity)` >>
+    drule_all generalise_0_FEMPTY >> simp[] >> strip_tac >>
+    `FDIFF gen_sub (msubst_vars sub mset) = gen_sub` by (
+      rw[fmap_eq_flookup, FLOOKUP_FDIFF] >> rw[FLOOKUP_DEF] >> gvs[]) >>
+    gvs[] >>
+    pop_assum kall_tac >>
+    qmatch_asmsub_abbrev_tac `gen_vars,_,let_ity` >>
+    `pure_vars (csubst (ishift gen_vars o_f closing) let_ity) = {}` by (
+      irule pure_vars_csubst_EMPTY_suff >> simp[GSYM IMAGE_FRANGE, PULL_EXISTS] >>
+      unabbrev_all_tac >> irule SUBSET_TRANS >>
+      irule_at Any pure_vars_pure_apply_subst_SUBSET >>
+      simp[GSYM IMAGE_FRANGE, IMAGE_IMAGE, combinTheory.o_DEF, pure_vars] >>
+      rw[IMAGE_K_EMPTY, DIFF_SUBSET] >>
+      qsuff_tac `pure_vars (pure_walkstar sub it1) ⊆ FDOM closing` >- rw[SUBSET_DEF] >>
+      simp[pure_vars_pure_walkstar_alt] >> rw[BIGUNION_SUBSET, PULL_EXISTS] >>
+      first_x_assum irule >> irule new_vars_SUBSET_minfer >>
+      qexistsl_tac [`as1`,`cs1`,`it1`] >> imp_res_tac minfer_pure_vars >>
+      simp[BIGUNION_FRANGE_maunion] >> simp[SUBSET_DEF, new_vars_def]) >>
+    pop_assum mp_tac >> simp[Once pure_vars_empty_eq_type_of] >> strip_tac >>
+    rename1 `SOME let_ty` >>
+    qexistsl_tac [`let_ty`,`gen_vars`,
+      `FUNION (DBVar o_f gen_sub) (ishift gen_vars o_f closing)`] >>
+    DEP_REWRITE_TAC[GSYM pure_apply_subst_FUNION] >>
+    simp[GSYM IMAGE_FRANGE, PULL_EXISTS, pure_vars] >> rw[]
+    >- (
+      irule ctxt_rel_sub >> goal_assum $ drule_at Any >>
+      simp[FLOOKUP_maunion] >> rw[] >> CASE_TAC >> simp[]
+      )
+    >- (
+      qsuff_tac `pure_vars (pure_walkstar sub (CVar n)) ⊆ FDOM closing`
+      >- rw[SUBSET_DEF] >>
+      first_x_assum irule >> irule new_vars_SUBSET_minfer >> goal_assum drule >>
+      simp[BIGUNION_FRANGE_maunion] >> imp_res_tac minfer_pure_vars >> simp[SUBSET_DEF]
+      )
+    >- (
+      pop_assum mp_tac >> qid_spec_tac `it` >>
+      ho_match_mp_tac IN_FRANGE_FUNION_suff >>
+      simp[GSYM IMAGE_FRANGE, PULL_EXISTS, pure_vars]
+      )
+    >- (
+      pop_assum mp_tac >> qid_spec_tac `it` >>
+      ho_match_mp_tac IN_FRANGE_FUNION_suff >>
+      simp[GSYM IMAGE_FRANGE, PULL_EXISTS, itype_ok, type_of_def] >>
+      rw[] >> last_x_assum drule >> rw[] >>
+      irule itype_ok_ishift >> simp[]
+      )
+    >- (
+      gvs[LIST_REL_EL_EQN] >> rw[EL_MAP] >> ntac 3 (pairarg_tac >> gvs[]) >>
+      first_x_assum drule >> simp[] >> PairCases_on `scheme` >> gvs[] >> rw[] >>
+      simp[o_f_FUNION] >> DEP_REWRITE_TAC[GSYM pure_apply_subst_FUNION] >>
+      simp[GSYM IMAGE_FRANGE, PULL_EXISTS, pure_vars] >>
+      qabbrev_tac `wlkit = pure_walkstar sub it` >>
+      `csubst ((ishift ivs o DBVar) o_f gen_sub) wlkit = wlkit` by (
+        irule pure_apply_subst_unchanged >> rw[DISJOINT_ALT, DISJ_EQ_IMP] >>
+        qpat_x_assum `msubst_vars _ _ = msubst_vars _ _` $ assume_tac o GSYM >>
+        simp[GSYM ctxt_vars_subst_ctxt] >>
+        simp[ctxt_vars_def, MEM_MAP, PULL_EXISTS, MEM_EL, EXISTS_PROD,
+             subst_ctxt_def, EL_MAP] >>
+        qpat_x_assum `_ ∈ pure_vars _` kall_tac >> unabbrev_all_tac >>
+        rpt $ goal_assum drule >> simp[]) >>
+      simp[] >> pop_assum kall_tac >>
+      irule shift_shift_let_lemma >> simp[] >>
+      unabbrev_all_tac >> irule SUBSET_TRANS >>
+      irule_at Any freedbvars_pure_walkstar_SUBSET >>
+      simp[BIGUNION_SUBSET, PULL_EXISTS] >>
+      gvs[EVERY_EL, itype_ok_def] >> first_x_assum drule >> simp[]
+      ) >>
+    last_x_assum irule >> rpt $ goal_assum drule >> simp[] >>
+    qexists_tac `(x,gen_vars,let_ity)::ictxt` >> simp[] >>
+    `pure_walkstar sub let_ity = let_ity` by (
+      unabbrev_all_tac >>
+      DEP_REWRITE_TAC[pure_walkstar_pure_apply_subst_pure_walkstar] >>
+      simp[GSYM IMAGE_FRANGE, PULL_EXISTS, pure_vars]) >>
+    simp[] >> rw[]
+    >- (
+      first_x_assum irule >> pop_assum mp_tac >>
+      simp[new_vars_def, PULL_EXISTS, pure_vars, IN_FRANGE_FLOOKUP,
+           FLOOKUP_maunion, DOMSUB_FLOOKUP_THM, GSYM DISJ_ASSOC, get_massumptions_def] >>
+      rw[] >> simp[SF SFY_ss] >>
+      Cases_on `k = x` >> gvs[] >- metis_tac[] >>
+      disj1_tac >> Cases_on `FLOOKUP as1 k`
+      >- (qexistsl_tac [`s`,`k`] >> simp[])
+      >- (qexistsl_tac [`x' ∪ s`,`k`] >> simp[])
+      )
+    >- (
+      simp[GSYM ctxt_vars_subst_ctxt] >>
+      simp[subst_ctxt, ctxt_vars] >> simp[ctxt_vars_subst_ctxt] >>
+      irule SUBSET_ANTISYM >> simp[]
+      )
+    >- (
+      unabbrev_all_tac >> irule SUBSET_TRANS >>
+      irule_at Any freedbvars_pure_apply_subst_SUBSET >>
+      simp[GSYM IMAGE_FRANGE, IMAGE_IMAGE, combinTheory.o_DEF, freedbvars_def] >>
+      simp[BIGUNION_SUBSET, PULL_EXISTS] >>
+      irule SUBSET_TRANS >> irule_at Any freedbvars_pure_walkstar_SUBSET >> simp[] >>
+      simp[BIGUNION_SUBSET, PULL_EXISTS] >>
+      imp_res_tac minfer_itype_ok >> gvs[itype_ok_def]
+      ) >>
+    gvs[ctxt_rel_def] >> reverse $ rw[]
+    >- (
+      first_x_assum $ qspec_then `k` mp_tac >>
+      simp[FLOOKUP_maunion, DOMSUB_FLOOKUP_THM] >>
+      every_case_tac >> gvs[] >> rw[] >> simp[]
+      ) >>
+    unabbrev_all_tac >>
+    gvs[DISJ_IMP_THM, IMP_CONJ_THM, FORALL_AND_THM, PULL_EXISTS] >>
+    gvs[get_massumptions_def, satisfies_def] >>
+    last_x_assum drule >> strip_tac >> simp[] >>
+    qabbrev_tac `wlkit1 = pure_walkstar sub it1` >>
+    qspecl_then [`gen_sub`,`sub'`,`wlkit1`] mp_tac pure_apply_subst_split_isubst >>
+    simp[] >> impl_tac >> rw[]
+    >- (
+      unabbrev_all_tac >> once_rewrite_tac[GSYM SUBSET_EMPTY] >>
+      irule SUBSET_TRANS >> irule_at Any freedbvars_pure_walkstar_SUBSET >>
+      simp[DISJ_EQ_IMP, IMAGE_EQ_SING] >>
+      imp_res_tac minfer_itype_ok >> gvs[itype_ok_def]
+      ) >>
+    goal_assum $ drule_at Any >> simp[EVERY_GENLIST] >> rw[]
+    >- (irule itype_ok_pure_apply_subst >> simp[itype_ok]) >>
+    simp[pure_vars_pure_apply_subst] >>
+    simp[SUBSET_DEF, pure_vars, PULL_EXISTS] >> rw[] >>
+    goal_assum drule >> qsuff_tac `gm ' n' ∈ FDOM gen_sub` >- simp[] >>
+    gvs[fmap_linv_alt_def, IN_FRANGE_FLOOKUP, FLOOKUP_DEF] >>
+    goal_assum drule >> simp[]
+    )
+  >- ( (* Letrec *)
+    gvs[DISJ_IMP_THM, FORALL_AND_THM, PULL_EXISTS, MAP2_MAP, MEM_MAP, MEM_ZIP] >>
+    simp[Once type_tcexp_cases] >> `fns ≠ []` by (CCONTR_TAC >> gvs[]) >> simp[] >>
+    last_x_assum $ irule_at Any >> goal_assum $ drule_at Any >> simp[] >>
+    `∃smonos : num_set. domain smonos = msubst_vars sub mset ∧ wf smonos` by (
+      qexists_tac `list_to_num_set (SET_TO_LIST (msubst_vars sub mset))` >>
+      simp[EXTENSION, domain_list_to_num_set, wf_list_to_num_set] >>
+      DEP_REWRITE_TAC[MEM_SET_TO_LIST] >> simp[msubst_vars_def, PULL_EXISTS]) >>
+    qabbrev_tac `gens =
+      MAP (generalise 0 smonos FEMPTY) (MAP (pure_walkstar sub) tys)` >>
+    `LIST_REL (λ(new,sub,ty) t.
+      CARD (FDOM sub) = new ∧ FDOM sub = pure_vars t DIFF domain smonos ∧
+      FRANGE sub = count new ∧ pure_vars ty ⊆ domain smonos ∧
+      csubst (DBVar o_f sub) t = ty)
+      gens (MAP (pure_walkstar sub) tys)` by (
+      unabbrev_all_tac >> rw[LIST_REL_EL_EQN, EL_MAP] >>
+      pairarg_tac >> simp[] >> drule generalise_0_FEMPTY >> simp[] >> rw[] >>
+      qsuff_tac `FDIFF sub' (msubst_vars sub mset) = sub'` >> rw[] >>
+      rw[fmap_eq_flookup, FLOOKUP_FDIFF] >> rw[FLOOKUP_DEF] >> gvs[]) >>
+    `EVERY (λit. pure_vars it = {}) $
+      MAP (λ(new,gen_sub,ty). csubst (ishift new o_f closing) ty) gens` by (
+      gvs[LIST_REL_EL_EQN, EVERY_EL, EL_MAP] >> rw[] >> pairarg_tac >> gvs[] >>
+      irule pure_vars_csubst_EMPTY_suff >> simp[GSYM IMAGE_FRANGE, PULL_EXISTS] >>
+      first_x_assum drule >> rw[] >>
+      irule SUBSET_TRANS >> irule_at Any pure_vars_pure_apply_subst_SUBSET >>
+      simp[GSYM IMAGE_FRANGE, IMAGE_IMAGE, combinTheory.o_DEF, pure_vars] >>
+      rw[IMAGE_K_EMPTY, DIFF_SUBSET] >>
+      qsuff_tac `pure_vars (pure_walkstar sub (EL n tys)) ⊆ FDOM closing`
+      >- rw[SUBSET_DEF] >>
+      simp[pure_vars_pure_walkstar_alt] >> rw[BIGUNION_SUBSET, PULL_EXISTS] >>
+      first_x_assum irule >>
+      simp[new_vars_def, MEM_MAP, MEM_EL, PULL_EXISTS, SF SFY_ss]) >>
+    pop_assum mp_tac >> simp[Once pure_vars_empty_eq_type_of_MAP] >> strip_tac >>
+    rename1 `MAP SOME fn_tys` >>
+    qexists_tac `ZIP (MAP FST gens, fn_tys)` >>
+    qexists_tac
+      `REVERSE (ZIP (MAP FST fns, MAP (λ(vs,s,t). (vs,t)) gens)) ++ ictxt` >> simp[] >>
+    imp_res_tac LIST_REL_LENGTH >> imp_res_tac $ cj 1 $ iffLR MAP_EQ_EVERY2 >> gvs[] >>
+    simp[AC (GSYM CONJ_ASSOC) CONJ_COMM] >> rw[]
+    >- (
+      first_x_assum irule >> pop_assum mp_tac >>
+      simp[new_vars_def, PULL_EXISTS, MEM_MAP, MEM_ZIP] >> rw[] >> gvs[SF SFY_ss] >>
+      gvs[IN_FRANGE_FLOOKUP, PULL_EXISTS, FLOOKUP_FDIFF, FLOOKUP_maunion] >>
+      Cases_on `¬MEM k (MAP FST fns)` >> gvs[GSYM DISJ_ASSOC]
+      >- (
+        disj1_tac >> simp[Once SWAP_EXISTS_THM] >>
+        qexists_tac `k` >> simp[] >> CASE_TAC >> simp[]
+        ) >>
+      ntac 4 disj2_tac >> disj1_tac >>
+      pop_assum mp_tac >> simp[MEM_MAP, MEM_EL, EXISTS_PROD] >> rw[] >>
+      pop_assum $ assume_tac o GSYM >> goal_assum $ drule_at Any >> simp[] >>
+      simp[PULL_EXISTS, pure_vars, get_massumptions_def, FLOOKUP_maunion] >>
+      qexists_tac `n` >> simp[] >> CASE_TAC >> simp[]
+      )
+    >- (
+      drule type_of_SOME_MAP >> rw[] >>
+      gvs[EVERY_EL, EL_ZIP, EL_MAP, LIST_REL_EL_EQN, MAP_EQ_EVERY2] >> rw[] >>
+      simp[GSYM itype_ok_type_ok] >>
+      ntac 3 (first_x_assum drule >> simp[] >> strip_tac) >>
+      pairarg_tac >> gvs[] >>
+      irule itype_ok_pure_apply_subst >>
+      simp[GSYM IMAGE_FRANGE, PULL_EXISTS] >> rw[]
+      >- (irule itype_ok_ishift >> simp[]) >>
+      irule itype_ok_pure_apply_subst >>
+      simp[GSYM IMAGE_FRANGE, PULL_EXISTS] >> rw[itype_ok] >>
+      irule itype_ok_pure_walkstar >> rw[] >- gvs[itype_ok_def] >>
+      last_x_assum drule >> simp[] >> pairarg_tac >> simp[] >> strip_tac >>
+      imp_res_tac minfer_itype_ok >> gvs[itype_ok_def]
+      )
+    >- (
+      gvs[ctxt_rel_def] >> rw[] >> simp[ALOOKUP_APPEND] >> CASE_TAC >> gvs[]
+      >- (
+        `¬MEM k (MAP FST fns)` by (
+          pop_assum mp_tac >>
+          simp[ALOOKUP_NONE, MEM_MAP, MEM_ZIP, PULL_EXISTS, EXISTS_PROD] >>
+          simp[Once MONO_NOT_EQ] >> rw[MEM_EL] >> csimp[EL_MAP] >>
+          goal_assum $ drule_at Any >> pop_assum $ assume_tac o GSYM >>
+          simp[] >> pairarg_tac >> simp[]) >>
+        first_x_assum $ qspec_then `k` mp_tac >> simp[FLOOKUP_FDIFF] >>
+        qsuff_tac
+         `∃v'. FLOOKUP (maunion as' (FOLDR maunion FEMPTY ass)) k = SOME v' ∧ v ⊆ v'`
+        >- (strip_tac >> simp[] >> rw[] >> gvs[SUBSET_DEF]) >>
+        simp[FLOOKUP_maunion] >> CASE_TAC >> simp[]
+        ) >>
+      PairCases_on `x` >> gvs[] >>
+      imp_res_tac ALOOKUP_MEM >> gvs[MEM_ZIP, MEM_MAP, EL_MAP] >>
+      pairarg_tac >> gvs[] >> rw[] >>
+      first_x_assum $ drule_at Any >>
+      pairarg_tac >> simp[PULL_EXISTS] >>
+      simp[get_massumptions_def, FLOOKUP_maunion] >> gvs[] >>
+      disch_then $ qspec_then `n'` mp_tac >> impl_tac >- (CASE_TAC >> simp[]) >>
+      simp[satisfies_def] >> rw[] >> simp[] >>
+      gvs[LIST_REL_EL_EQN] >> first_x_assum drule >> simp[EL_MAP] >> rw[] >>
+      DEP_REWRITE_TAC[pure_walkstar_pure_apply_subst_pure_walkstar] >>
+      simp[GSYM IMAGE_FRANGE, PULL_EXISTS, pure_vars] >>
+      qabbrev_tac `wlk = pure_walkstar sub (EL n tys)` >>
+      qspecl_then [`s`,`sub'`,`wlk`] mp_tac pure_apply_subst_split_isubst >>
+      simp[] >> impl_tac >> rw[]
+      >- (
+        unabbrev_all_tac >> once_rewrite_tac[GSYM SUBSET_EMPTY] >>
+        irule SUBSET_TRANS >> irule_at Any freedbvars_pure_walkstar_SUBSET >>
+        simp[DISJ_EQ_IMP, IMAGE_EQ_SING] >>
+        last_x_assum drule >> simp[EL_ZIP] >> strip_tac >>
+        imp_res_tac minfer_itype_ok >> gvs[itype_ok_def]
+        ) >>
+      goal_assum $ drule_at Any >> simp[EVERY_GENLIST] >> rw[]
+      >- (irule itype_ok_pure_apply_subst >> simp[itype_ok]) >>
+      simp[pure_vars_pure_apply_subst] >>
+      simp[SUBSET_DEF, pure_vars, PULL_EXISTS] >> rw[] >>
+      goal_assum drule >> qsuff_tac `gm ' n'' ∈ FDOM s` >- simp[] >>
+      gvs[fmap_linv_alt_def, IN_FRANGE_FLOOKUP, FLOOKUP_DEF] >>
+      goal_assum drule >> simp[]
+      )
+    >- (
+      simp[ctxt_vars, msubst_vars_UNION] >> irule SUBSET_ANTISYM >> simp[] >>
+      simp[GSYM ctxt_vars_subst_ctxt] >>
+      simp[subst_ctxt_def, ctxt_vars_def,
+           ZIP_MAP, MAP_MAP_o, combinTheory.o_DEF, LAMBDA_PROD] >>
+      simp[BIGUNION_SUBSET, PULL_EXISTS, MEM_MAP, MEM_ZIP] >> rw[] >>
+      pairarg_tac >> simp[] >> pairarg_tac >> simp[] >>
+      gvs[LIST_REL_EL_EQN, EL_MAP] >> first_x_assum drule >> simp[] >> rw[] >>
+      pairarg_tac >> gvs[] >>
+      DEP_REWRITE_TAC[pure_walkstar_pure_apply_subst_pure_walkstar] >>
+      simp[GSYM IMAGE_FRANGE, PULL_EXISTS, pure_vars]
+      )
+    >- (
+      gvs[EVERY_EL, EL_ZIP, EL_MAP] >> rw[] >>
+      pairarg_tac >> gvs[] >> pairarg_tac >> gvs[] >>
+      gvs[LIST_REL_EL_EQN, EL_MAP] >> first_x_assum drule >> simp[] >> strip_tac >>
+      pop_assum $ assume_tac o GSYM >> simp[] >>
+      irule SUBSET_TRANS >> irule_at Any freedbvars_pure_apply_subst_SUBSET >>
+      simp[GSYM IMAGE_FRANGE, IMAGE_IMAGE, combinTheory.o_DEF, freedbvars_def] >>
+      reverse conj_tac >- simp[SUBSET_DEF, PULL_EXISTS] >>
+      irule SUBSET_TRANS >> irule_at Any freedbvars_pure_walkstar_SUBSET >> simp[] >>
+      simp[BIGUNION_SUBSET, PULL_EXISTS] >> reverse conj_tac >- gvs[itype_ok_def] >>
+      last_x_assum drule >> simp[EL_ZIP] >> pairarg_tac >> simp[] >> strip_tac >>
+      imp_res_tac minfer_itype_ok >> gvs[itype_ok_def]
+      )
+    >- (
+      gvs[LIST_REL_EL_EQN, MAP_EQ_EVERY2, EL_ZIP, EL_MAP] >> rw[] >>
+      simp[EL_APPEND_EQN] >> CASE_TAC >> gvs[] >>
+      simp[EL_REVERSE, EL_ZIP, EL_MAP, LAMBDA_PROD] >>
+      qmatch_goalsub_abbrev_tac `EL m` >>
+      `m < LENGTH fn_tys` by (unabbrev_all_tac >> gvs[]) >>
+      rpt (pairarg_tac >> gvs[]) >>
+      first_x_assum drule >> simp[] >>
+      qsuff_tac `pure_walkstar sub it' = it'` >> rw[] >>
+      first_x_assum drule >> simp[] >>
+      rw[] >> DEP_REWRITE_TAC[pure_walkstar_pure_apply_subst_pure_walkstar] >>
+      simp[GSYM IMAGE_FRANGE, PULL_EXISTS, pure_vars]
+      ) >>
+    gvs[LIST_REL_EL_EQN, MAP_EQ_EVERY2, EL_ZIP, EL_MAP] >> rw[] >>
+    pairarg_tac >> gvs[] >> pairarg_tac >> gvs[] >>
+    last_assum drule >> asm_rewrite_tac[] >> simp[] >>
+    strip_tac >> pop_assum irule >> conj_tac
+    >- (
+      rw[] >> qpat_x_assum `∀c s. _ ∧ MEM _ __ ⇒ _` irule >>
+      goal_assum $ drule_at Any >> simp[EL_MEM]
+      ) >>
+    first_assum drule >> pairarg_tac >> asm_rewrite_tac[] >> rw[] >>
+    qpat_assum `∀n. n < _ ⇒ _ (pure_walkstar _ _)` drule >>
+    asm_rewrite_tac[] >> simp[] >> strip_tac >> gvs[] >>
+    qmatch_asmsub_abbrev_tac `EL n gens = (new,gen_sub,ty)` >>
+    qexists_tac `FUNION (DBVar o_f gen_sub) (ishift new o_f closing)` >>
+    qexists_tac `REVERSE (ZIP (MAP FST fns, MAP (λ(vs,s,t). (vs,t)) gens)) ++ ictxt` >>
+    simp[] >> rw[]
+    >- (
+      pop_assum mp_tac >> qid_spec_tac `it'` >>
+      ho_match_mp_tac IN_FRANGE_FUNION_suff >>
+      simp[GSYM IMAGE_FRANGE, PULL_EXISTS, pure_vars]
+      )
+    >- (
+      pop_assum mp_tac >> qid_spec_tac `it'` >>
+      ho_match_mp_tac IN_FRANGE_FUNION_suff >>
+      simp[GSYM IMAGE_FRANGE, PULL_EXISTS, itype_ok] >> rw[] >>
+      irule itype_ok_ishift >> gvs[itype_ok_def]
+      )
+    >- (
+      simp[EL_APPEND_EQN] >> reverse $ rw[] >> simp[EL_MAP, EL_REVERSE, EL_ZIP]
+      >- (
+        qmatch_goalsub_abbrev_tac `EL m`  >>
+        `m < LENGTH ictxt` by (unabbrev_all_tac >> gvs[]) >>
+        rpt (pairarg_tac >> gvs[]) >>
+        qpat_x_assum `∀n. _ < LENGTH ictxt ⇒ _` $ qspec_then `m` mp_tac >> rw[] >>
+        simp[o_f_FUNION] >> DEP_REWRITE_TAC[GSYM pure_apply_subst_FUNION] >>
+        simp[GSYM IMAGE_FRANGE, PULL_EXISTS, ishift_def, pure_vars] >>
+        `csubst ((ishift ivs o DBVar) o_f gen_sub) (pure_walkstar sub it') =
+          pure_walkstar sub it'` by (
+          irule pure_apply_subst_unchanged >> simp[] >> rw[DISJOINT_ALT] >>
+          disj2_tac >> qpat_x_assum `msubst_vars _ _ = _` $ assume_tac o GSYM >>
+          simp[GSYM ctxt_vars_subst_ctxt, subst_ctxt_def, ctxt_vars_def] >>
+          simp[MEM_MAP, PULL_EXISTS, EXISTS_PROD, MEM_EL] >>
+          goal_assum drule >> goal_assum $ drule_at Any o GSYM >> simp[]) >>
+        pop_assum SUBST_ALL_TAC >> irule shift_shift_let_lemma >> simp[] >>
+        irule SUBSET_TRANS >> irule_at Any freedbvars_pure_walkstar_SUBSET >>
+        simp[BIGUNION_SUBSET, PULL_EXISTS] >> gvs[EVERY_EL, itype_ok_def] >>
+        qpat_x_assum `∀n. n < LENGTH ictxt ⇒ _` $ qspec_then `m` mp_tac >> simp[]
+        )
+      >- (
+        qmatch_goalsub_abbrev_tac `EL m`  >>
+        `m < LENGTH fn_tys` by (unabbrev_all_tac >> gvs[]) >>
+        rpt (pairarg_tac >> gvs[]) >>
+        first_x_assum drule >> rw[] >> first_x_assum drule >> rw[] >>
+        DEP_REWRITE_TAC[pure_walkstar_pure_apply_subst_pure_walkstar] >>
+        simp[GSYM IMAGE_FRANGE, PULL_EXISTS, pure_vars] >>
+        qmatch_goalsub_abbrev_tac `ishift new'` >>
+        simp[o_f_FUNION] >> DEP_REWRITE_TAC[GSYM pure_apply_subst_FUNION] >>
+        simp[GSYM IMAGE_FRANGE, PULL_EXISTS, ishift_def, pure_vars] >>
+        `csubst ((ishift new' ∘ DBVar) o_f gen_sub) $
+          csubst (DBVar o_f s) (pure_walkstar sub (EL m tys)) =
+          csubst (DBVar o_f s) (pure_walkstar sub (EL m tys))` by (
+          irule pure_apply_subst_unchanged >> rw[DISJOINT_ALT] >>
+          disj2_tac >> pop_assum mp_tac >>
+          simp[pure_vars_pure_apply_subst] >>
+          csimp[PULL_EXISTS, pure_vars, pure_apply_subst, FLOOKUP_DEF] >>
+          gen_tac >> CASE_TAC >> simp[pure_vars] >> rw[]) >>
+        pop_assum $ SUBST_ALL_TAC >> irule shift_shift_let_lemma >> gvs[] >>
+        irule SUBSET_TRANS >> irule_at Any freedbvars_pure_apply_subst_SUBSET >>
+        simp[GSYM IMAGE_FRANGE, IMAGE_IMAGE, combinTheory.o_DEF, freedbvars_def] >>
+        reverse conj_tac >- (rw[SUBSET_DEF] >> gvs[]) >>
+        irule SUBSET_TRANS >> irule_at Any freedbvars_pure_walkstar_SUBSET >>
+        simp[] >> reverse conj_tac >- gvs[BIGUNION_SUBSET, PULL_EXISTS, itype_ok_def] >>
+        last_x_assum drule >> simp[] >> strip_tac >>
+        imp_res_tac minfer_itype_ok >> gvs[itype_ok_def]
+        )
+      )
+    >- (
+      qsuff_tac `pure_vars (pure_walkstar sub (CVar n')) ⊆ FDOM closing`
+      >- rw[SUBSET_DEF] >>
+      first_x_assum irule >> pop_assum mp_tac >>
+      simp[new_vars_def, MEM_MAP, MEM_ZIP, PULL_EXISTS, IN_FRANGE_FLOOKUP,
+           FLOOKUP_FDIFF, FLOOKUP_maunion, GSYM DISJ_ASSOC, FORALL_PROD] >>
+      reverse $ rw[]
+      >- simp[MEM_EL, PULL_EXISTS, SF SFY_ss]
+      >- simp[MEM_EL, PULL_EXISTS, SF SFY_ss] >>
+      Cases_on `¬MEM k (MAP FST fns)` >> gvs[]
+      >- (
+        gvs[MEM_MAP, FORALL_PROD] >> disj1_tac >>
+        simp[Once SWAP_EXISTS_THM] >> qexists_tac `k` >> simp[] >>
+        qsuff_tac `∃v. FLOOKUP (FOLDR maunion FEMPTY ass) k = SOME v ∧ s ⊆ v`
+        >- (rw[] >> simp[] >> CASE_TAC >> gvs[SUBSET_DEF]) >>
+        simp[FLOOKUP_FOLDR_maunion, MEM_EL, PULL_EXISTS] >>
+        goal_assum $ drule_at Any >>
+        gvs[FLOOKUP_DEF, SUBSET_DEF, PULL_EXISTS, SF SFY_ss]
+        ) >>
+      ntac 4 disj2_tac >> disj1_tac >>
+      pop_assum mp_tac >> simp[MEM_MAP, EXISTS_PROD, MEM_EL] >> rw[] >>
+      goal_assum $ drule_at Any >> pop_assum $ assume_tac o GSYM >>
+      simp[get_massumptions_def, FLOOKUP_maunion, PULL_EXISTS, pure_vars] >>
+      qexists_tac `n'` >> simp[] >>
+      qsuff_tac `∃v. FLOOKUP (FOLDR maunion FEMPTY ass) k = SOME v ∧ s ⊆ v`
+      >- (rw[] >> simp[] >> CASE_TAC >> gvs[SUBSET_DEF]) >>
+      simp[FLOOKUP_FOLDR_maunion, MEM_EL, PULL_EXISTS] >>
+      qexists_tac `n` >> gvs[FLOOKUP_DEF, SUBSET_DEF, PULL_EXISTS, SF SFY_ss]
+      )
+    >- (
+      simp[ctxt_vars, msubst_vars_UNION] >> irule SUBSET_ANTISYM >> simp[] >>
+      simp[GSYM ctxt_vars_subst_ctxt] >>
+      simp[subst_ctxt_def, ctxt_vars_def,
+           ZIP_MAP, MAP_MAP_o, combinTheory.o_DEF, LAMBDA_PROD] >>
+      simp[BIGUNION_SUBSET, PULL_EXISTS, MEM_MAP, MEM_ZIP] >> rw[] >>
+      pairarg_tac >> simp[] >> pairarg_tac >> simp[] >>
+      gvs[LIST_REL_EL_EQN, EL_MAP] >> first_x_assum drule >> simp[] >> rw[] >>
+      pairarg_tac >> gvs[] >>
+      first_x_assum drule >> simp[] >> rw[] >>
+      DEP_REWRITE_TAC[pure_walkstar_pure_apply_subst_pure_walkstar] >>
+      simp[GSYM IMAGE_FRANGE, PULL_EXISTS, pure_vars]
+      )
+    >- (
+      DEP_REWRITE_TAC[GSYM pure_apply_subst_FUNION] >>
+      simp[GSYM IMAGE_FRANGE, PULL_EXISTS, pure_vars]
+      )
+    >- (
+      gvs[EVERY_EL, EL_ZIP, EL_MAP] >> rw[] >>
+      pairarg_tac >> gvs[] >> pairarg_tac >> gvs[] >>
+      first_x_assum drule >> simp[] >> strip_tac >>
+      first_x_assum drule >> simp[] >> rw[] >>
+      irule SUBSET_TRANS >> irule_at Any freedbvars_pure_apply_subst_SUBSET >>
+      simp[GSYM IMAGE_FRANGE, IMAGE_IMAGE, combinTheory.o_DEF, freedbvars_def] >>
+      reverse conj_tac >- simp[SUBSET_DEF, PULL_EXISTS] >>
+      irule SUBSET_TRANS >> irule_at Any freedbvars_pure_walkstar_SUBSET >> simp[] >>
+      simp[BIGUNION_SUBSET, PULL_EXISTS] >> reverse conj_tac >- gvs[itype_ok_def] >>
+      last_x_assum drule >> simp[EL_ZIP] >> pairarg_tac >> simp[] >> strip_tac >>
+      imp_res_tac minfer_itype_ok >> gvs[itype_ok_def]
+      )
+    >- (
+      gvs[ctxt_rel_def] >> rw[] >> simp[ALOOKUP_APPEND] >> CASE_TAC >> gvs[]
+      >- (
+        `¬MEM k (MAP FST fns)` by (
+          pop_assum mp_tac >>
+          simp[ALOOKUP_NONE, MEM_MAP, MEM_ZIP, PULL_EXISTS, EXISTS_PROD] >>
+          simp[Once MONO_NOT_EQ] >> rw[MEM_EL] >> csimp[EL_MAP] >>
+          goal_assum $ drule_at Any >> pop_assum $ assume_tac o GSYM >>
+          simp[] >> pairarg_tac >> simp[]) >>
+        first_x_assum $ qspec_then `k` mp_tac >> simp[FLOOKUP_FDIFF] >>
+        qsuff_tac
+         `∃v'. FLOOKUP (maunion as' (FOLDR maunion FEMPTY ass)) k = SOME v' ∧ v ⊆ v'`
+        >- (strip_tac >> simp[] >> rw[] >> gvs[SUBSET_DEF]) >>
+        simp[FLOOKUP_maunion, FLOOKUP_FOLDR_maunion, MEM_EL, PULL_EXISTS] >>
+        IF_CASES_TAC >> gvs[]
+        >- (first_x_assum $ qspec_then `n` assume_tac >> gvs[FLOOKUP_DEF])
+        >- (CASE_TAC >> simp[SUBSET_DEF, PULL_EXISTS, SF SFY_ss])
+        ) >>
+      PairCases_on `x` >> gvs[] >>
+      imp_res_tac ALOOKUP_MEM >> gvs[MEM_ZIP, MEM_MAP, EL_MAP] >>
+      pairarg_tac >> gvs[] >> rw[] >>
+      qabbrev_tac `n'_fns = EL n' fns` >> PairCases_on `n'_fns` >> gvs[] >>
+      qpat_x_assum `∀c n. _ ⇒ satisifes _ _ _` $ drule_at Any >>
+      simp[PULL_EXISTS, get_massumptions_def] >>
+      `∃v'. FLOOKUP (maunion as' (FOLDR maunion FEMPTY ass)) n'_fns0 =
+              SOME v' ∧ v ⊆ v'` by (
+        simp[FLOOKUP_maunion, FLOOKUP_FOLDR_maunion, MEM_EL, PULL_EXISTS] >>
+        IF_CASES_TAC >> gvs[]
+        >- (first_x_assum $ qspec_then `n` assume_tac >> gvs[FLOOKUP_DEF]) >>
+        CASE_TAC >> simp[SUBSET_DEF, PULL_EXISTS, SF SFY_ss]) >>
+      simp[satisfies_def] >> disch_then $ qspec_then `n''` mp_tac >>
+      impl_tac >- gvs[SUBSET_DEF] >> rw[] >>
+      qpat_x_assum `∀n. _ ⇒ _ (pure_walkstar _ _)` drule >> rw[] >>
+      DEP_REWRITE_TAC[pure_walkstar_pure_apply_subst_pure_walkstar] >>
+      simp[GSYM IMAGE_FRANGE, PULL_EXISTS, pure_vars] >>
+      qabbrev_tac `wlk = pure_walkstar sub (EL n' tys)` >>
+      qspecl_then [`s`,`sub'`,`wlk`] mp_tac pure_apply_subst_split_isubst >>
+      simp[] >> impl_tac >> rw[]
+      >- (
+        unabbrev_all_tac >> once_rewrite_tac[GSYM SUBSET_EMPTY] >>
+        irule SUBSET_TRANS >> irule_at Any freedbvars_pure_walkstar_SUBSET >>
+        simp[DISJ_EQ_IMP, IMAGE_EQ_SING] >>
+        last_x_assum drule >> simp[EL_ZIP] >> strip_tac >>
+        imp_res_tac minfer_itype_ok >> gvs[itype_ok_def]
+        ) >>
+      goal_assum $ drule_at Any >> simp[EVERY_GENLIST] >> rw[]
+      >- (irule itype_ok_pure_apply_subst >> simp[itype_ok]) >>
+      rename1 `gm ' foo` >>
+      simp[pure_vars_pure_apply_subst] >>
+      simp[SUBSET_DEF, pure_vars, PULL_EXISTS] >> rw[] >>
+      goal_assum drule >> qsuff_tac `gm ' foo ∈ FDOM s` >- simp[] >>
+      gvs[fmap_linv_alt_def, IN_FRANGE_FLOOKUP, FLOOKUP_DEF] >>
+      goal_assum drule >> simp[]
+      )
+    )
+  >- ( (* BoolCase *)
+    simp[Once type_tcexp_cases] >> disj1_tac >>
+    gvs[DISJ_IMP_THM, FORALL_AND_THM, PULL_EXISTS, satisfies_def] >>
+    gvs[pure_walkstar_alt, pure_apply_subst, type_of_def] >>
+    gvs[GSYM pure_walkstar_alt] >>
+    ntac 3 $ last_x_assum $ irule_at Any >>
+    ntac 5 $ goal_assum $ drule_at Any >> simp[] >>
+    qexistsl_tac [`(v,0,BoolTy)::ictxt`,`(v,0,BoolTy)::ictxt`] >> simp[] >>
+    simp[freedbvars_def, pure_walkstar_alt, pure_apply_subst, type_of_def] >>
+    simp[GSYM pure_walkstar_alt] >> simp[ctxt_vars, pure_vars] >> rw[]
+    >- (
+      irule ctxt_rel_sub >> goal_assum $ drule_at Any >> rw[] >>
+      simp[FLOOKUP_maunion] >> CASE_TAC >> simp[]
+      )
+    >- (
+      first_x_assum irule >> irule new_vars_SUBSET_minfer >> goal_assum drule >>
+      simp[BIGUNION_FRANGE_maunion] >> imp_res_tac minfer_pure_vars >> simp[SUBSET_DEF]
+      )
+    >- (
+      gvs[ctxt_rel_def, get_massumptions_def] >> rw[] >- simp[pure_walkstar_alt] >>
+      first_x_assum $ qspec_then `k` mp_tac >>
+      simp[FLOOKUP_maunion, DOMSUB_FLOOKUP_THM] >>
+      every_case_tac >> rw[] >> gvs[]
+      )
+    >- (
+      first_x_assum irule >> pop_assum mp_tac >>
+      simp[new_vars_def, PULL_EXISTS, pure_vars, IN_FRANGE_FLOOKUP, FLOOKUP_maunion,
+           DOMSUB_FLOOKUP_THM, GSYM DISJ_ASSOC, get_massumptions_def] >>
+      rw[] >> simp[SF SFY_ss] >>
+      Cases_on `n = f` >> gvs[] >> simp[SF SFY_ss] >>
+      Cases_on `v = k` >> gvs[] >> simp[SF SFY_ss] >> disj1_tac >>
+      simp[Once SWAP_EXISTS_THM] >> qexists_tac `k` >> simp[] >>
+      every_case_tac >> simp[]
+      )
+    >- (
+      gvs[ctxt_rel_def, get_massumptions_def] >> rw[] >- simp[pure_walkstar_alt] >>
+      first_x_assum $ qspec_then `k` mp_tac >>
+      simp[FLOOKUP_maunion, DOMSUB_FLOOKUP_THM] >>
+      every_case_tac >> rw[] >> gvs[]
+      )
+    >- (
+      first_x_assum irule >> pop_assum mp_tac >>
+      simp[new_vars_def, PULL_EXISTS, pure_vars, IN_FRANGE_FLOOKUP, FLOOKUP_maunion,
+           DOMSUB_FLOOKUP_THM, GSYM DISJ_ASSOC, get_massumptions_def] >>
+      rw[] >> simp[SF SFY_ss] >>
+      Cases_on `n = f` >> gvs[] >> simp[SF SFY_ss] >>
+      Cases_on `v = k` >> gvs[] >> simp[SF SFY_ss] >> disj1_tac >>
+      simp[Once SWAP_EXISTS_THM] >> qexists_tac `k` >> simp[] >>
+      every_case_tac >> simp[]
+      )
+    )
+  >- ( (* TupleCase *)
+    simp[Once type_tcexp_cases] >> disj1_tac >>
+    gvs[DISJ_IMP_THM, FORALL_AND_THM, PULL_EXISTS, LEFT_AND_OVER_OR, MAP2_MAP,
+        MEM_MAP, MEM_ZIP, EL_MAP, satisfies_def] >>
+    gvs[pure_walkstar_alt, pure_apply_subst] >> gvs[GSYM $ cj 9 pure_walkstar_alt] >>
+    last_x_assum $ irule_at $ Pos hd >> rpt $ goal_assum $ drule_at Any >> simp[] >>
+    irule_at Any $ cj 1 type_of_lemma >>
+    `EVERY (λit. pure_vars it = {}) $
+      MAP (csubst closing) $ MAP (pure_walkstar sub) $ MAP CVar freshes` by (
+        rw[EVERY_MAP, EVERY_MEM] >> irule pure_vars_csubst_EMPTY_suff >> simp[] >>
+        first_x_assum irule >> simp[new_vars_def, pure_vars, MEM_MAP, PULL_EXISTS]) >>
+    gvs[pure_vars_empty_eq_type_of_MAP] >> irule_at Any EQ_REFL >> rw[]
+    >- (
+      irule ctxt_rel_sub >> goal_assum $ drule_at Any >> rw[] >>
+      simp[FLOOKUP_maunion] >> CASE_TAC >> simp[]
+      )
+    >- (
+      first_x_assum irule >> irule new_vars_SUBSET_minfer >> goal_assum drule >>
+      simp[BIGUNION_FRANGE_maunion] >> imp_res_tac minfer_pure_vars >> simp[SUBSET_DEF]
+      )
+    >- gvs[MAP_EQ_EVERY2] >>
+    last_x_assum irule >> goal_assum $ drule_at Any >> simp[] >>
+    qexists_tac `REVERSE (ZIP (pvars,MAP ($, 0) (MAP CVar freshes))) ++
+                  (v,0,CVar f)::ictxt` >>
+    simp[freedbvars_def, LIST_TO_SET_MAP, IMAGE_EQ_SING, PULL_EXISTS] >> rw[]
+    >- (
+      first_x_assum irule >> pop_assum mp_tac >>
+      simp[new_vars_def, PULL_EXISTS, pure_vars, IN_FRANGE_FLOOKUP,
+           FLOOKUP_maunion, FLOOKUP_FDIFF, GSYM DISJ_ASSOC, get_massumptions_def,
+           MEM_MAP, MEM_ZIP, EL_MAP] >>
+      rw[] >> simp[SF SFY_ss] >>
+      Cases_on `n = f` >> gvs[] >> simp[SF SFY_ss] >>
+      Cases_on `v = k` >> gvs[] >> simp[SF SFY_ss] >>
+      Cases_on `MEM k pvars`
+      >- (
+        gvs[MEM_EL] >> ntac 5 disj2_tac >> disj1_tac >>
+        qexistsl_tac [`n'`,`n`] >> simp[]
+        ) >>
+      disj1_tac >> simp[Once SWAP_EXISTS_THM] >> qexists_tac `k` >> simp[] >>
+      CASE_TAC >> simp[]
+      )
+    >- (
+      simp[ctxt_vars, pure_vars, msubst_vars_UNION] >>
+      simp[GSYM msubst_vars_UNION] >> AP_TERM_TAC >>
+      once_rewrite_tac[INSERT_SING_UNION] >> rewrite_tac[UNION_ASSOC] >>
+      AP_THM_TAC >> AP_TERM_TAC >> simp[Once UNION_COMM] >> AP_TERM_TAC >>
+      simp[ctxt_vars_def, Once EXTENSION, MEM_MAP, MEM_ZIP,
+           MEM_EL, PULL_EXISTS, EL_MAP, SF CONJ_ss, pure_vars] >>
+      rw[] >> eq_tac >> rw[] >> goal_assum $ drule_at Any >> simp[]
+      )
+    >- (rw[EVERY_MEM, MEM_ZIP, MEM_MAP] >> simp[EL_MAP, freedbvars_def])
+    >- (
+      irule EVERY2_APPEND_suff >> simp[] >>
+      simp[pure_apply_subst] >> irule_at Any $ cj 1 type_of_lemma >> simp[] >>
+      gvs[LIST_REL_EL_EQN, MAP_EQ_EVERY2, EL_ZIP, EL_MAP]
+      )
+    >- (
+      gvs[ctxt_rel_def] >> rw[] >> gvs[ALOOKUP_APPEND, get_massumptions_def] >>
+      reverse $ TOP_CASE_TAC >> simp[]
+      >- (
+        PairCases_on `x` >> rw[] >>
+        imp_res_tac ALOOKUP_MEM >> gvs[MEM_ZIP, MEM_MAP, EL_MAP]
+        ) >>
+      IF_CASES_TAC >> gvs[] >> first_x_assum $ qspec_then `k` mp_tac >>
+      simp[FLOOKUP_maunion, FLOOKUP_FDIFF] >>
+      gvs[ALOOKUP_NONE, MEM_MAP, MEM_ZIP, EL_MAP, PULL_EXISTS] >>
+      IF_CASES_TAC >- gvs[MEM_EL] >> simp[] >>
+      TOP_CASE_TAC >> gvs[] >> rw[] >> simp[]
+      )
+    )
+  >- ( (* ExceptionCase *)
+    simp[Once type_tcexp_cases] >> ntac 2 disj2_tac >> disj1_tac >>
+    gvs[DISJ_IMP_THM, FORALL_AND_THM, PULL_EXISTS, MEM_MAP, satisfies_def] >>
+    gvs[pure_walkstar_alt, pure_apply_subst] >> gvs[GSYM pure_walkstar_alt] >>
+    PairCases_on `ns` >> gvs[] >>
+    last_x_assum $ irule_at Any >> rpt $ goal_assum $ drule_at Any >>
+    rw[type_of_def]
+    >- (
+      irule ctxt_rel_sub >> goal_assum $ drule_at Any >> rw[] >>
+      simp[FLOOKUP_maunion] >> CASE_TAC >> simp[]
+      )
+    >- (
+      first_x_assum irule >> irule new_vars_SUBSET_minfer >> goal_assum drule >>
+      simp[BIGUNION_FRANGE_maunion] >> imp_res_tac minfer_pure_vars >> simp[SUBSET_DEF]
+      )
+    >- (
+      imp_res_tac sortingTheory.PERM_LIST_TO_SET >> gvs[] >>
+      qspec_then `FST` drule sortingTheory.PERM_MAP >> rw[] >>
+      drule sortingTheory.PERM_LIST_TO_SET >>
+      simp[MAP_MAP_o, combinTheory.o_DEF, LAMBDA_PROD, FST_THM]
+      )
+    >- (imp_res_tac sortingTheory.PERM_LENGTH >> gvs[]) >>
+    gvs[LIST_REL_EL_EQN, EVERY_EL, EL_ZIP, EL_MAP] >> rw[] >>
+    pairarg_tac >> gvs[] >> pairarg_tac >> gvs[] >>
+    first_x_assum drule >> simp[] >> strip_tac >> simp[] >>
+    `c ≠ "Subscript"` by (
+      qpat_x_assum `namespace_ok _` assume_tac >>
+      gvs[namespace_ok_def, ALL_DISTINCT_APPEND] >>
+      last_x_assum $ qspec_then `"Subscript"` mp_tac >>
+      impl_tac >- simp[pure_configTheory.reserved_cns_def] >> strip_tac >>
+      CCONTR_TAC >> gvs[] >> imp_res_tac ALOOKUP_MEM >> gvs[MEM_MAP]) >>
+    simp[] >> rpt conj_asm1_tac
+    >- (
+      gvs[MEM_FLAT, MEM_MAP, DISJ_EQ_IMP, PULL_EXISTS, EXISTS_PROD, MEM_EL] >>
+      metis_tac[]
+      )
+    >- (
+      gvs[namespace_ok_def, ALL_DISTINCT_APPEND] >>
+      qsuff_tac `MEM (c, LENGTH pvars) (MAP (λ(cn,ts). (cn, LENGTH ts)) ns0)`
+      >- (
+        rw[] >> gvs[MEM_MAP, EXISTS_PROD] >>
+        rev_drule ALOOKUP_ALL_DISTINCT_MEM >> disch_then drule >> simp[]
+        ) >>
+      drule $ iffRL sortingTheory.PERM_MEM_EQ >>
+      simp[MEM_MAP, EXISTS_PROD, PULL_EXISTS, FORALL_PROD] >>
+      simp[Once MEM_EL, PULL_EXISTS] >> disch_then drule >> simp[]
+      ) >>
+    last_x_assum drule >> simp[] >> strip_tac >> pop_assum irule >> conj_tac
+    >- (
+      gvs[MEM_EL, PULL_EXISTS] >> rw[] >>
+      first_x_assum irule >> goal_assum drule >> simp[]
+      ) >>
+    goal_assum $ drule_at Any >> simp[] >>
+    qexists_tac `REVERSE (ZIP (pvars,MAP ($, 0) (MAP itype_of schemes))) ++
+                  (v,0,CVar f)::ictxt` >>
+    qpat_x_assum `∀c s. _ ∧ _ ⇒ _` mp_tac >> simp[Once MEM_EL, PULL_EXISTS] >>
+    disch_then $ drule_at Any >>
+    simp[PULL_EXISTS, MAP2_MAP, MEM_MAP, MEM_ZIP,
+         DISJ_IMP_THM, FORALL_AND_THM, satisfies_def, EL_MAP] >>
+    strip_tac >> gvs[] >> rw[]
+    >- (
+      simp[EL_APPEND_EQN, EL_REVERSE, EL_ZIP, EL_MAP] >>
+      reverse $ rw[] >- (Cases_on `n' - LENGTH pvars` >> gvs[freedbvars_def]) >>
+      gvs[namespace_ok_def, EVERY_EL, freetyvars_ok_freedbvars] >>
+      drule ALOOKUP_MEM >> simp[MEM_EL] >> strip_tac >> pop_assum $ assume_tac o GSYM >>
+      last_x_assum drule >> simp[] >>
+      disch_then $ qspec_then `PRE (LENGTH pvars − n')` mp_tac >>
+      simp[GSYM itype_ok_type_ok, itype_ok_def]
+      )
+    >- (
+      simp[EL_APPEND_EQN, EL_REVERSE, EL_ZIP, EL_MAP] >> rw[type_of_itype_of] >>
+      Cases_on `n' - LENGTH pvars` >> gvs[pure_apply_subst, type_of_def]
+      )
+    >- (
+      first_x_assum irule >> reverse $ gvs[new_vars_def] >>
+      simp[pure_vars, PULL_EXISTS, MEM_MAP, GSYM DISJ_ASSOC]
+      >- (
+        Cases_on `n` >> gvs[] >>
+        ntac 4 disj2_tac >> disj1_tac >> irule_at Any OR_INTRO_THM2 >>
+        goal_assum drule >> simp[EL] >> DEP_REWRITE_TAC[EL_MEM] >>
+        gvs[namespace_ok_def] >> Cases_on `tys` >> gvs[]
+        )
+      >- (
+        ntac 6 disj2_tac >> disj1_tac >>
+        simp[MEM_EL, PULL_EXISTS] >> rpt $ goal_assum $ drule_at Any >> simp[]
+        ) >>
+      gvs[IN_FRANGE_FLOOKUP, FLOOKUP_maunion, FLOOKUP_FOLDR_maunion] >>
+      Cases_on `k ∈ v INSERT set pvars` >> gvs[]
+      >- (
+        ntac 6 disj2_tac >> disj1_tac >> simp[MEM_EL, PULL_EXISTS] >>
+        goal_assum $ drule_at Any >> simp[PULL_EXISTS] >>
+        rpt $ irule_at Any OR_INTRO_THM1 >> simp[PULL_EXISTS, pure_vars] >>
+        simp[get_massumptions_def] >> goal_assum drule >> simp[]
+        )
+      >- (
+        ntac 6 disj2_tac >> disj1_tac >> simp[MEM_EL, PULL_EXISTS] >>
+        goal_assum $ drule_at Any >> simp[PULL_EXISTS] >>
+        irule_at Any OR_INTRO_THM1 >> irule_at Any OR_INTRO_THM2 >>
+        simp[PULL_EXISTS, MAP2_MAP, MEM_MAP, MEM_ZIP, EL_MAP, pure_vars] >>
+        gvs[MEM_EL] >> qexists_tac `n''` >> simp[] >>
+        simp[get_massumptions_def] >> goal_assum drule >> simp[]
+        )
+      >- (
+        rpt disj1_tac >> simp[PULL_EXISTS, Once SWAP_EXISTS_THM] >>
+        qexists_tac `k` >> CASE_TAC >> gvs[]
+        >- (
+          irule FALSITY >> pop_assum mp_tac >> simp[MEM_EL, PULL_EXISTS] >>
+          goal_assum drule >> gvs[FLOOKUP_DEF]
+          ) >>
+        CASE_TAC >> simp[PULL_EXISTS, MEM_EL] >> gvs[]
+        >- (rpt $ goal_assum $ drule_at Any >> simp[FLOOKUP_FDIFF])
+        >- (disj2_tac >> rpt $ goal_assum $ drule_at Any >> simp[FLOOKUP_FDIFF])
+        )
+      )
+    >- (
+      simp[ctxt_vars, msubst_vars_UNION] >> simp[GSYM msubst_vars_UNION] >>
+      AP_TERM_TAC >> simp[pure_vars, UNION_ASSOC] >>
+      once_rewrite_tac[INSERT_SING_UNION] >> AP_THM_TAC >> AP_TERM_TAC >>
+      simp[ctxt_vars_def, MAP_REVERSE, ZIP_MAP, MAP_MAP_o, combinTheory.o_DEF,
+           LAMBDA_PROD, LIST_TO_SET_MAP] >>
+      rw[Once EXTENSION, PULL_EXISTS, EXISTS_PROD]
+      )
+    >- (
+      Cases_on `n` >> gvs[] >> simp[EL] >>
+      qpat_x_assum `∀t. MEM _ _ ⇒ _` $ qspec_then `EL n' (TL tys)` mp_tac >>
+      impl_tac >> rw[] >> gvs[] >> irule EL_MEM >> Cases_on `tys` >> gvs[]
+      )
+    >- (
+      gvs[ctxt_rel_def] >> rw[] >> gvs[ALOOKUP_APPEND, get_massumptions_def] >>
+      reverse $ TOP_CASE_TAC >> simp[]
+      >- (
+        PairCases_on `x` >> rw[] >>
+        imp_res_tac ALOOKUP_MEM >> gvs[MEM_ZIP, MEM_MAP, EL_MAP]
+        ) >>
+      IF_CASES_TAC >> gvs[] >>
+      first_x_assum $ qspec_then `k` mp_tac >> simp[FLOOKUP_maunion] >>
+      qsuff_tac
+        `∃s. FLOOKUP (FOLDR maunion FEMPTY final_as) k = SOME s ∧ v' ⊆ s`
+      >- (strip_tac >> simp[] >> CASE_TAC >> rw[] >> gvs[SUBSET_DEF]) >>
+      `¬ MEM k pvars` by (
+        qpat_x_assum `ALOOKUP _ _ = _` mp_tac >>
+        simp[ALOOKUP_NONE, MEM_MAP, FORALL_PROD, MEM_ZIP, EXISTS_PROD] >>
+        rw[Once MONO_NOT_EQ, MEM_EL] >> irule_at Any EQ_REFL >> simp[EL_MAP]) >>
+      simp[FLOOKUP_FOLDR_maunion] >> rw[MEM_EL, PULL_EXISTS]
+      >- (goal_assum drule >> gvs[FLOOKUP_DEF]) >>
+      simp[SUBSET_DEF, PULL_EXISTS] >> rw[] >>
+      rpt $ goal_assum drule >> simp[FLOOKUP_FDIFF]
+      )
+    )
+  >- ( (* Case *)
+    simp[Once type_tcexp_cases] >> rpt disj2_tac >>
+    gvs[DISJ_IMP_THM, FORALL_AND_THM, PULL_EXISTS, MEM_MAP, satisfies_def] >>
+    gvs[pure_walkstar_alt, pure_apply_subst] >> gvs[GSYM $ cj 9 pure_walkstar_alt] >>
+    PairCases_on `ns` >> gvs[] >>
+    last_x_assum $ irule_at Any >> rpt $ goal_assum $ drule_at Any >>
+    qexists_tac `id` >> simp[] >>
+    irule_at Any $ cj 2 type_of_lemma >>
+    `EVERY (λit. pure_vars it = {}) $ MAP (csubst closing) $
+      MAP (pure_walkstar sub) $ MAP CVar freshes` by (
+      rw[EVERY_MEM, MEM_MAP] >> irule pure_vars_csubst_EMPTY_suff >> simp[] >>
+      first_x_assum irule >> simp[new_vars_def, pure_vars, MEM_MAP, PULL_EXISTS]) >>
+    gvs[pure_vars_empty_eq_type_of_MAP] >> irule_at Any EQ_REFL >>
+    imp_res_tac $ cj 1 $ iffLR MAP_EQ_EVERY2 >> gvs[] >> rw[]
+    >- (
+      irule ctxt_rel_sub >> goal_assum $ drule_at Any >> rw[] >>
+      simp[FLOOKUP_maunion] >> CASE_TAC >> simp[]
+      )
+    >- (
+      first_x_assum irule >> irule new_vars_SUBSET_minfer >> goal_assum drule >>
+      simp[BIGUNION_FRANGE_maunion] >> imp_res_tac minfer_pure_vars >> simp[SUBSET_DEF]
+      )
+    >- (
+      imp_res_tac sortingTheory.PERM_LIST_TO_SET >> gvs[] >>
+      qspec_then `FST` drule sortingTheory.PERM_MAP >> rw[] >>
+      drule sortingTheory.PERM_LIST_TO_SET >>
+      simp[MAP_MAP_o, combinTheory.o_DEF, LAMBDA_PROD, FST_THM]
+      )
+    >- (imp_res_tac sortingTheory.PERM_LENGTH >> gvs[]) >>
+    gvs[LIST_REL_EL_EQN, EVERY_EL, EL_ZIP, EL_MAP] >> rw[] >>
+    pairarg_tac >> gvs[] >> pairarg_tac >> gvs[] >>
+    first_x_assum drule >> simp[] >> strip_tac >> simp[] >> rpt conj_asm1_tac
+    >- (
+      gvs[namespace_ok_def, ALL_DISTINCT_APPEND] >>
+      `MEM (c, LENGTH pvars) (MAP (λ(cn,ts). (cn, LENGTH ts)) cdefs)` by (
+        drule $ iffRL sortingTheory.PERM_MEM_EQ >>
+        simp[MEM_MAP, EXISTS_PROD, PULL_EXISTS, FORALL_PROD] >>
+        disch_then irule >> simp[MEM_EL] >> goal_assum drule >> simp[]) >>
+      gvs[MEM_MAP, EXISTS_PROD] >>
+      drule_at (Pos last) ALOOKUP_ALL_DISTINCT_MEM >> impl_tac >> simp[] >>
+      gvs[MAP_FLAT, MAP_MAP_o, combinTheory.o_DEF, LAMBDA_PROD] >>
+      irule ALL_DISTINCT_FLAT_IMP >> goal_assum drule >>
+      simp[MEM_MAP, EXISTS_PROD] >> irule_at Any EQ_REFL >> simp[MEM_EL] >>
+      gvs[oEL_THM] >> goal_assum drule >> simp[]
+      )
+    >- (
+      gvs[MEM_FLAT, MEM_MAP, DISJ_EQ_IMP, PULL_EXISTS, EXISTS_PROD, MEM_EL] >>
+      metis_tac[]
+      ) >>
+    last_x_assum drule >> simp[] >> strip_tac >> pop_assum irule >> conj_tac
+    >- (
+      gvs[MEM_EL, PULL_EXISTS] >> rw[] >>
+      first_x_assum irule >> goal_assum drule >> simp[]
+      ) >>
+    goal_assum $ drule_at Any >> simp[] >>
+    qexists_tac `REVERSE (ZIP (pvars,MAP ($, 0)
+      (MAP (isubst (MAP CVar freshes) o itype_of) schemes))) ++ (v,0,CVar f)::ictxt` >>
+    qpat_x_assum `∀c s. _ ∧ _ ⇒ _` mp_tac >> simp[Once MEM_EL, PULL_EXISTS] >>
+    disch_then $ drule_at Any >>
+    simp[PULL_EXISTS, MAP2_MAP, MEM_MAP, MEM_ZIP,
+         DISJ_IMP_THM, FORALL_AND_THM, satisfies_def, EL_MAP] >>
+    strip_tac >> gvs[] >> rw[]
+    >- (
+      simp[EL_APPEND_EQN, EL_REVERSE, EL_ZIP, EL_MAP] >>
+      reverse $ rw[] >- (Cases_on `n' - LENGTH schemes` >> gvs[freedbvars_def]) >>
+      gvs[namespace_ok_def, EVERY_EL, freetyvars_ok_freedbvars, oEL_THM] >>
+      drule ALOOKUP_MEM >> simp[MEM_EL] >> strip_tac >> pop_assum $ assume_tac o GSYM >>
+      last_x_assum kall_tac >> last_x_assum drule >> simp[] >>
+      disch_then drule >> simp[] >>
+      disch_then $ qspec_then `PRE (LENGTH schemes − n')` mp_tac >>
+      rw[GSYM itype_ok_type_ok, itype_ok_def] >>
+      irule freedbvars_isubst_EMPTY_suff >> simp[EVERY_MAP, freedbvars_def]
+      )
+    >- (
+      simp[EL_APPEND_EQN, EL_REVERSE, EL_ZIP, EL_MAP] >> rw[type_of_itype_of]
+      >- (
+        DEP_REWRITE_TAC[pure_walkstar_isubst] >> conj_tac >- gvs[itype_ok_def] >>
+        simp[pure_apply_subst_isubst_itype_of] >>
+        drule_then (assume_tac o GSYM) type_of_SOME_MAP >>
+        simp[isubst_itype_of, type_of_itype_of]
+        )
+      >- (
+        Cases_on `n' - LENGTH schemes` >> gvs[pure_apply_subst] >>
+        irule $ cj 2 type_of_lemma >> simp[]
+        )
+      )
+    >- (
+      first_x_assum irule >> reverse $ gvs[new_vars_def] >>
+      simp[pure_vars, PULL_EXISTS, MEM_MAP, GSYM DISJ_ASSOC]
+      >- (
+        Cases_on `n` >> gvs[] >>
+        ntac 5 disj2_tac >> disj1_tac >> irule_at Any OR_INTRO_THM2 >>
+        goal_assum drule >> simp[EL] >> DEP_REWRITE_TAC[EL_MEM] >>
+        gvs[namespace_ok_def] >> Cases_on `tys` >> gvs[]
+        )
+      >- (
+        ntac 7 disj2_tac >> disj1_tac >>
+        simp[MEM_EL, PULL_EXISTS] >> rpt $ goal_assum $ drule_at Any >> simp[]
+        ) >>
+      gvs[IN_FRANGE_FLOOKUP, FLOOKUP_maunion, FLOOKUP_FOLDR_maunion] >>
+      Cases_on `k ∈ v INSERT set pvars` >> gvs[]
+      >- (
+        ntac 7 disj2_tac >> disj1_tac >> simp[MEM_EL, PULL_EXISTS] >>
+        goal_assum $ drule_at Any >> simp[PULL_EXISTS] >>
+        rpt $ irule_at Any OR_INTRO_THM1 >> simp[PULL_EXISTS, pure_vars] >>
+        simp[get_massumptions_def] >> goal_assum drule >> simp[]
+        )
+      >- (
+        ntac 7 disj2_tac >> disj1_tac >> simp[MEM_EL, PULL_EXISTS] >>
+        goal_assum $ drule_at Any >> simp[PULL_EXISTS] >>
+        irule_at Any OR_INTRO_THM1 >> irule_at Any OR_INTRO_THM2 >>
+        simp[PULL_EXISTS, MAP2_MAP, MEM_MAP, MEM_ZIP, EL_MAP, pure_vars] >>
+        gvs[MEM_EL] >> qexists_tac `n''` >> simp[] >>
+        simp[get_massumptions_def] >> goal_assum drule >> simp[]
+        )
+      >- (
+        rpt disj1_tac >> simp[PULL_EXISTS, Once SWAP_EXISTS_THM] >>
+        qexists_tac `k` >> CASE_TAC >> gvs[]
+        >- (
+          irule FALSITY >> pop_assum mp_tac >> simp[MEM_EL, PULL_EXISTS] >>
+          goal_assum drule >> gvs[FLOOKUP_DEF]
+          ) >>
+        CASE_TAC >> simp[PULL_EXISTS, MEM_EL] >> gvs[]
+        >- (rpt $ goal_assum $ drule_at Any >> simp[FLOOKUP_FDIFF])
+        >- (disj2_tac >> rpt $ goal_assum $ drule_at Any >> simp[FLOOKUP_FDIFF])
+        )
+      )
+    >- (
+      once_rewrite_tac[INSERT_SING_UNION] >> rewrite_tac[msubst_vars_UNION] >>
+      simp[ctxt_vars, msubst_vars_UNION, pure_vars, UNION_ASSOC] >>
+      AP_THM_TAC >> AP_TERM_TAC >>
+      simp[msubst_vars_def, ctxt_vars_def, MAP_REVERSE, ZIP_MAP, MAP_MAP_o,
+           combinTheory.o_DEF, LAMBDA_PROD, LIST_TO_SET_MAP, IMAGE_IMAGE,
+           pure_vars] >>
+      irule SUBSET_ANTISYM >> simp[] >>
+      simp[SUBSET_DEF, PULL_EXISTS, MEM_ZIP] >> rw[] >>
+      qspecl_then [`MAP CVar freshes`,`itype_of (EL n' schemes)`]
+        mp_tac pure_vars_isubst_SUBSET >>
+      simp[MAP_MAP_o, combinTheory.o_DEF, pure_vars, LIST_TO_SET_MAP,
+           SUBSET_DEF, PULL_EXISTS] >>
+      disch_then drule >> simp[SF SFY_ss]
+      )
+    >- (
+      Cases_on `n` >> gvs[] >> simp[EL] >>
+      qpat_x_assum `∀t. MEM _ _ ⇒ _` $ qspec_then `EL n' (TL tys)` mp_tac >>
+      impl_tac >> rw[] >> gvs[] >> irule EL_MEM >> Cases_on `tys` >> gvs[]
+      )
+    >- (
+      gvs[ctxt_rel_def] >> rw[] >> gvs[ALOOKUP_APPEND, get_massumptions_def] >>
+      reverse $ TOP_CASE_TAC >> simp[]
+      >- (
+        PairCases_on `x` >> rw[] >>
+        imp_res_tac ALOOKUP_MEM >> gvs[MEM_ZIP, MEM_MAP, EL_MAP]
+        ) >>
+      IF_CASES_TAC >> gvs[] >>
+      first_x_assum $ qspec_then `k` mp_tac >> simp[FLOOKUP_maunion] >>
+      qsuff_tac
+        `∃s. FLOOKUP (FOLDR maunion FEMPTY final_as) k = SOME s ∧ v' ⊆ s`
+      >- (strip_tac >> simp[] >> CASE_TAC >> rw[] >> gvs[SUBSET_DEF]) >>
+      `¬ MEM k pvars` by (
+        qpat_x_assum `ALOOKUP _ _ = _` mp_tac >>
+        simp[ALOOKUP_NONE, MEM_MAP, FORALL_PROD, MEM_ZIP, EXISTS_PROD] >>
+        rw[Once MONO_NOT_EQ, MEM_EL] >> irule_at Any EQ_REFL >> simp[EL_MAP]) >>
+      simp[FLOOKUP_FOLDR_maunion] >> rw[MEM_EL, PULL_EXISTS]
+      >- (goal_assum drule >> gvs[FLOOKUP_DEF]) >>
+      simp[SUBSET_DEF, PULL_EXISTS] >> rw[] >>
+      rpt $ goal_assum drule >> simp[FLOOKUP_FDIFF]
+      )
+    )
+QED
+
 
 (****************************************)
 
